defined algorithmic subtyping, completeness proven but transitivity proof evasive

Subsumption-STLC.v
@@ -100,1353 +100,1392 @@ End IdDec.
 Module IS := WS.Make(IdDec).
 Module ISF := MSF.WFactsOn(IdDec)(IS).
 
-Definition field (t : Type) : Type := id * t.
+Section Fields.
+    Definition field (t : Type) : Type := id * t.
 
-Definition fields (t : Type) : Type := list (field t).
+    Definition fields (t : Type) : Type := list (field t).
 
-Definition predf {U : Type} (P : U -> Prop) (f : field U) : Prop := 
-    P (snd f).
+    Definition predf {U : Type} (P : U -> Prop) (f : field U) : Prop := 
+        P (snd f).
 
-Definition predf_prop {U : Type} {V : Prop} (P : U -> V) (f : field U) : V :=
-    P (snd f).
+    Definition predf_prop {U : Type} {V : Prop} (P : U -> V) (f : field U) : V :=
+        P (snd f).
 
-Definition predfs {U : Type} (P : U -> Prop) : fields U -> Prop := 
-    Forall (predf P).
+    Definition predfs {U : Type} (P : U -> Prop) : fields U -> Prop := 
+        Forall (predf P).
 
-Definition perm {U : Type} (u1 : fields U) (u2 : fields U) : Prop :=
-    Permutation u1 u2.
+    Definition perm {U : Type} (u1 : fields U) (u2 : fields U) : Prop :=
+        Permutation u1 u2.
 
-Definition relf {U V : Type} (R : U -> V -> Prop) (u : field U) (v : field V) : Prop :=
-    (fst u) = (fst v) /\ R (snd u) (snd v).
+    Definition relf {U V : Type} (R : U -> V -> Prop) (u : field U) (v : field V) : Prop :=
+        (fst u) = (fst v) /\ R (snd u) (snd v).
 
-Definition relfs {U V : Type} (R : U -> V -> Prop) : fields U -> fields V -> Prop :=
-    Forall2 (relf R).
+    Definition relfs {U V : Type} (R : U -> V -> Prop) : fields U -> fields V -> Prop :=
+        Forall2 (relf R).
 
-(* Coq doesn't let me use this but it would be helpful. *)
-Fixpoint fields_pred_ind {U : Type} {P : U -> Prop}
-(Q : forall (u : U), P u)
-(us : fields U) : predfs P us :=
-    match us as us' return (predfs P us') with
-    | [] => Forall_nil (predf P)
-    | h :: t => Forall_cons h
-        (Q (snd h))
-        (fields_pred_ind Q t)
-    end.
+    (* Coq doesn't let me use this but it would be helpful. *)
+    Fixpoint fields_pred_ind {U : Type} {P : U -> Prop}
+    (Q : forall (u : U), P u)
+    (us : fields U) : predfs P us :=
+        match us as us' return (predfs P us') with
+        | [] => Forall_nil (predf P)
+        | h :: t => Forall_cons h
+            (Q (snd h))
+            (fields_pred_ind Q t)
+        end.
 
-Definition relf_pred {U V : Type} 
-{R1 : U -> V -> Prop} {R2 : U -> V -> Prop}
-{u : field U} {v : field V}
-(Q : forall (u' : U) (v' : V), R1 u' v' -> R2 u' v')
-(H : relf R1 u v) :=
-    match H with
-    | conj Hname HR1 => conj Hname (Q (snd u) (snd v) HR1)
-    end.
+    Definition relf_pred {U V : Type} 
+    {R1 : U -> V -> Prop} {R2 : U -> V -> Prop}
+    {u : field U} {v : field V}
+    (Q : forall (u' : U) (v' : V), R1 u' v' -> R2 u' v')
+    (H : relf R1 u v) :=
+        match H with
+        | conj Hname HR1 => conj Hname (Q (snd u) (snd v) HR1)
+        end.
 
-(* record field names must be unique *)
-Definition nodupfs {U : Type} (us : fields U) : Prop :=
-    NoDup (map fst us).
+    (* record field names must be unique *)
+    Definition nodupfs {U : Type} (us : fields U) : Prop :=
+        NoDup (map fst us).
 
-Lemma relfs_name_share :
-    forall {U V : Type} (R : U -> V -> Prop)
-    (us : fields U) (vs : fields V) (x : id),
-    relfs R us vs ->
-    In x (map fst us) <-> In x (map fst vs).
-Proof.
-    intros U V R us vs x HR. 
-    induction HR; split; intros HI; inv HI;
-    destruct x0 as [x0 ux0]; destruct y as [y vy];
-    destruct H as [Hfst Hr]; simpl in *; subst;
-    try (left; reflexivity);
-    destruct HI as [HYX | HXIN];
-    try (left; assumption);
-    try (right; apply IHHR; assumption).
-Qed.
+    Lemma relfs_name_share :
+        forall {U V : Type} (R : U -> V -> Prop)
+        (us : fields U) (vs : fields V) (x : id),
+        relfs R us vs ->
+        In x (map fst us) <-> In x (map fst vs).
+    Proof.
+        intros U V R us vs x HR. 
+        induction HR; split; intros HI; inv HI;
+        destruct x0 as [x0 ux0]; destruct y as [y vy];
+        destruct H as [Hfst Hr]; simpl in *; subst;
+        try (left; reflexivity);
+        destruct HI as [HYX | HXIN];
+        try (left; assumption);
+        try (right; apply IHHR; assumption).
+    Qed.
 
-Lemma relfs_in_fst :
-    forall {U : Type} (us : fields U) (x : id) (u : U),
-    In (x, u) us -> In x (map fst us).
-Proof.
-    intros U us x u H. induction us; inv H;
-    simpl in *.
-    - left. reflexivity.
-    - destruct a as [a au]; simpl in *.
-        destruct H as [H | H].
-        + injintrosubst H. left. reflexivity.
-        + right. auto.
-Qed.
+    Lemma relfs_in_fst :
+        forall {U : Type} (us : fields U) (x : id) (u : U),
+        In (x, u) us -> In x (map fst us).
+    Proof.
+        intros U us x u H. induction us; inv H;
+        simpl in *.
+        - left. reflexivity.
+        - destruct a as [a au]; simpl in *.
+            destruct H as [H | H].
+            + injintrosubst H. left. reflexivity.
+            + right. auto.
+    Qed.
 
-Lemma relfs_nodup_eq :
-    forall {U : Type} (us : fields U) (x : id) (u1 u2 : U),
-    nodupfs us -> 
-    In (x,u1) us -> In (x,u2) us -> u1 = u2.
-Proof.
-    intros U us x u1 u2 ND H1 H2.
-    induction us; inv H1; inv H2; inv ND.
-    - injintrosubst H. reflexivity.
-    - apply IHus; auto. exfalso.
-        apply H4. apply relfs_in_fst in H. assumption.
-    - apply IHus; auto. exfalso.
-        apply H4. apply relfs_in_fst in H. assumption.
-    - apply IHus; auto.
-Qed.
+    Lemma relfs_nodup_eq :
+        forall {U : Type} (us : fields U) (x : id) (u1 u2 : U),
+        nodupfs us -> 
+        In (x,u1) us -> In (x,u2) us -> u1 = u2.
+    Proof.
+        intros U us x u1 u2 ND H1 H2.
+        induction us; inv H1; inv H2; inv ND.
+        - injintrosubst H. reflexivity.
+        - apply IHus; auto. exfalso.
+            apply H4. apply relfs_in_fst in H. assumption.
+        - apply IHus; auto. exfalso.
+            apply H4. apply relfs_in_fst in H. assumption.
+        - apply IHus; auto.
+    Qed.
 
-Lemma relfs_app :
-    forall {U V : Type} (R : U -> V -> Prop) 
-    (us1 us2 : fields U) (vs : fields V),
-    relfs R (us1 ++ us2) vs ->
-    exists (vs1 vs2 : fields V),
-    vs = vs1 ++ vs2 /\
-    relfs R us1 vs1 /\ relfs R us2 vs2.
-Proof.
-    intros U V R us1 us2 vs HR.
-    apply Forall2_app_inv_l in HR.
-    destruct HR as [vs1 [vs2 [H1 [H2 Hvs]]]].
-    exists vs1. exists vs2. auto.
-Qed.
+    Lemma relfs_app :
+        forall {U V : Type} (R : U -> V -> Prop) 
+        (us1 us2 : fields U) (vs : fields V),
+        relfs R (us1 ++ us2) vs ->
+        exists (vs1 vs2 : fields V),
+        vs = vs1 ++ vs2 /\
+        relfs R us1 vs1 /\ relfs R us2 vs2.
+    Proof.
+        intros U V R us1 us2 vs HR.
+        apply Forall2_app_inv_l in HR.
+        destruct HR as [vs1 [vs2 [H1 [H2 Hvs]]]].
+        exists vs1. exists vs2. auto.
+    Qed.
 
-Lemma relfs_app_dist :
-    forall {U V : Type} (R : U -> V -> Prop)
-    (us1 us2 : fields U) (vs1 vs2 : fields V),
-    relfs R us1 vs1 -> relfs R us2 vs2 ->
-    relfs R (us1 ++ us2) (vs1 ++ vs2).
-Proof.
-    intros U V R us1 us2 vs1 vs2 HR1 HR2.
-    apply Forall2_app; auto.
-Qed.
+    Lemma relfs_app_dist :
+        forall {U V : Type} (R : U -> V -> Prop)
+        (us1 us2 : fields U) (vs1 vs2 : fields V),
+        relfs R us1 vs1 -> relfs R us2 vs2 ->
+        relfs R (us1 ++ us2) (vs1 ++ vs2).
+    Proof.
+        intros U V R us1 us2 vs1 vs2 HR1 HR2.
+        apply Forall2_app; auto.
+    Qed.
+
+    Lemma relfs_in_exists_r :
+        forall {U V : Type} (R : U -> V -> Prop)
+        (us : fields U) (vs : fields V) (v : field V),
+        In v vs ->
+        relfs R us vs ->
+        exists (u : field U), In u us /\
+        relf R u v.
+    Proof.
+        intros U V R us vs v Hinvs HRusvs.
+        induction HRusvs; inv Hinvs.
+        - exists x. split; auto.
+            apply in_eq.
+        - apply IHHRusvs in H0 as [u [Hinl HRuv]].
+            exists u. split; auto.
+            apply in_cons; auto.
+    Qed.
+
+    Lemma relfs_in_exists_l :
+        forall {U V : Type} (R : U -> V -> Prop)
+        (us : fields U) (vs : fields V) (u : field U),
+        In u us ->
+        relfs R us vs ->
+        exists (v : field V), In v vs /\
+        relf R u v.
+    Proof.
+        intros U V R us vs u Hinus HRusvs.
+        induction HRusvs; inv Hinus.
+        - exists y. split; auto.
+            apply in_eq.
+        - apply IHHRusvs in H0 as [v [Hinl HRuv]].
+            exists v. split; auto.
+            apply in_cons; auto.
+    Qed.
+End Fields.
 
 Module SubsumptionSTLC.
-Inductive type : Type :=
-    | TTop
-    | TUnit
-    | TFun (t t' : type)
-    | TRec (fs : fields type).
-
-Definition fields_type := fields type.
-
-(* Doesn't work because Coq's Scheme Command is stupid :
-    To use Scheme the Types must be mutually defined 
-    with the "with" keyword. *)
-Fail Scheme type_rec' := Induction for type Sort Type
-    with fields_type_rec := Induction for fields_type Sort Type.
-
-(* automatically generated induction principle is weak *)
-Check type_ind.
-Compute type_ind.
-Compute type_rect.
-
-(* custom induction principle for Type type *)
-Section TypeInduction.
-    Variable P : type -> Prop.
-
-    Hypothesis HTop : P TTop.
-
-    Hypothesis HUnit : P TUnit.
-
-    Hypothesis HFun : forall (t t' : type),
-        P t -> P t' -> P (TFun t t').
-
-    Hypothesis HRec : forall (fs : fields type),
-        predfs P fs -> P (TRec fs).
-
-    Fixpoint IHType (t : type) : P t :=
-        match t as ty return P ty with 
-        | TTop => HTop
-        | TUnit => HUnit
-        | TFun t1 t2 => HFun t1 t2 (IHType t1) (IHType t2)
-        | TRec fs =>
-            let fix list_ih (fs' : fields type) : predfs P fs' :=
-                match fs' as fs_ty return predfs P fs_ty with
-                | [] => Forall_nil (predf P)
-                | hf :: tf => Forall_cons hf (IHType (snd hf)) (list_ih tf)
-                end in
-            HRec fs (list_ih fs)
-        end.
-End TypeInduction.
-
-Ltac indtype t := induction t using IHType.
-
-(* The Subtyping Relation *)
-Inductive subtype : type -> type -> Prop :=
-    | st_refl : forall (t : type), 
-        subtype t t
-    | st_trans : forall (t u v : type),
-        subtype t u -> 
-        subtype u v ->
-        subtype t v
-    | st_top : forall (t : type),
-        subtype t TTop
-    | st_fun : forall (u u' v v' : type),
-        subtype u' u ->
-        subtype v v' ->
-        subtype (TFun u v) (TFun u' v')
-    | st_rec_width : forall (us vs : fields type),
-        subtype (TRec (us ++ vs)) (TRec us)
-    | st_rec_depth : forall (us vs : fields type),
-        relfs subtype us vs ->
-        subtype (TRec us) (TRec vs)
-    | st_rec_perm : forall (us vs : fields type),
-        perm us vs ->
-        subtype (TRec us) (TRec vs).
-
-Check subtype_ind.
-Compute subtype_ind.
-
-Section SubtypeInduction.
-    Variable P : type -> type -> Prop.
-
-    Hypothesis HRefl : forall (t : type), P t t.
-
-    Hypothesis HTrans : forall (t u v : type),
-        subtype t u -> P t u ->
-        subtype u v -> P u v -> P t v.
-
-    Hypothesis HTop : forall (t : type), P t TTop.
-
-    Hypothesis HFun : forall (u u' v v' : type),
-        subtype u' u -> P u' u ->
-        subtype v v' -> P v v' ->
-        P (TFun u v) (TFun u' v').
-
-    Hypothesis HRecWidth : forall (us vs : fields type),
-        P (TRec (us ++ vs)) (TRec us).
-
-    Hypothesis HRecDepth : forall (us vs : fields type),
-        relfs subtype us vs -> relfs P us vs ->
-        P (TRec us) (TRec vs).
-
-    Hypothesis HRecPerm : forall (us vs : fields type),
-        perm us vs -> P (TRec us) (TRec vs).
-    
-    Fixpoint IHSubtype (t t' : type) (HS : subtype t t') {struct HS} : P t t' :=
-        match HS in (subtype w w') return (P w w') with
-        | st_refl t => HRefl t
-        | st_trans t u v Htu Huv =>
-            HTrans t u v Htu (IHSubtype t u Htu) Huv (IHSubtype u v Huv)
-        | st_top t => HTop t
-        | st_fun u u' v v' Hu Hv =>
-            HFun u u' v v' Hu (IHSubtype u' u Hu) Hv (IHSubtype v v' Hv)
-        | st_rec_width us vs => HRecWidth us vs
-        | st_rec_depth us vs HRs =>
-            let fix depth_helper {us' : fields type} {vs' : fields type}
-                (HRs' : relfs subtype us' vs') : Forall2 (relf P) us' vs' :=
-                match HRs' in (Forall2 _ lu lv) 
-                    return (Forall2 (relf P) lu lv) with
-                | Forall2_nil _ => Forall2_nil (relf P)
-                | Forall2_cons u v Huv Husvs =>
-                    Forall2_cons
-                        u v (relf_pred IHSubtype Huv) 
-                        (depth_helper Husvs)
-                end in
-            HRecDepth us vs HRs (depth_helper HRs) 
-        | st_rec_perm us vs HP => HRecPerm us vs HP
-        end.
-End SubtypeInduction.
-
-Lemma st_fields_refl :
-    forall (fs : fields type), relfs subtype fs fs.
-Proof. induction fs; constructor.
-    - split; constructor.
-    - assumption.
-Qed.
-
-Lemma st_fields_rec :
-    forall (us vs : fields type),
-    relfs subtype us vs -> subtype (TRec us) (TRec vs).
-Proof.
-    intros us vs HS. constructor. assumption.
-Qed.
-
-Example record_subtyping_makes_sense :
-    subtype 
-        (TRec [("x",TUnit);("y",TUnit)]) 
-        (TRec [("y",TTop)]).
-Proof.
-    apply st_trans with (u := TRec [("y",TUnit)]).
-    - apply st_trans with (u := TRec [("y", TUnit); ("x", TUnit)]).
-        + apply st_rec_perm. constructor.
-        + assert (HE : [("y", TUnit); ("x", TUnit)] 
-            = [("y", TUnit)] ++ [("x", TUnit)]);
-            try reflexivity. rewrite HE.
-            apply st_rec_width.
-    - apply st_rec_depth. constructor.
-        + split; auto. apply st_top.
-        + constructor.
-Qed.
-
-Inductive expr : Type :=
-    | EUnit
-    | EVar (x : id)
-    | EFun (x : id) (t : type) (e : expr)
-    | EApp (e1 e2 : expr)
-    | ERec (fs : fields expr)
-    | EPrj (e : expr) (x : id).
-
-(* custom induction principle for Type expr *)
-Section ExprInduction.
-    Variable P : expr -> Prop.
-
-    Hypothesis HUnit : P EUnit.
-
-    Hypothesis HVar : forall (x : id), P (EVar x).
-
-    Hypothesis HFun : forall (x : id) (t : type) (e : expr),
-        P e -> P (EFun x t e).
-
-    Hypothesis HApp : forall (e1 e2 : expr),
-        P e1 -> P e2 -> P (EApp e1 e2).
-
-    Hypothesis HRec : forall (fs : fields expr),
-        predfs P fs -> P (ERec fs).
-
-    Hypothesis HPrj : forall (e : expr) (x : id),
-        P e -> P (EPrj e x).
-
-    Check Forall_cons.
-
-    Fixpoint IHExpr (e : expr) : P e :=
-        match e as ee return (P ee) with
-        | EUnit => HUnit
-        | EVar x => HVar x
-        | EFun x t e => HFun x t e (IHExpr e)
-        | EApp e1 e2 => HApp e1 e2 (IHExpr e1) (IHExpr e2)
-        | ERec fs =>
-            let fix rec_help (fs' : fields expr) : predfs P fs' :=
-                match fs' as fs'' return (predfs P fs'') with
-                | [] => Forall_nil (predf P)
-                | hf::tf => Forall_cons hf (IHExpr (snd hf)) (rec_help tf)
-                end in
-            HRec fs (rec_help fs)
-        | EPrj e x => HPrj e x (IHExpr e)
-        end.
-End ExprInduction.
-
-Ltac indexpr e := induction e using IHExpr.
-
-(* Static Semantics with Subsumption *)
-Inductive check (g : gamma) : expr -> type -> Prop :=
-    | check_subsume : forall (e : expr) (u v : type),
-        subtype u v ->
-        check g e u ->
-        check g e v
-    | check_unit :
-        check g EUnit TUnit
-    | check_var : forall (x : id) (t : type),
-        g x = Some t ->
-        check g (EVar x) t
-    | check_fun : forall (x : id) (u v : type) (e : expr),
-        check (bind x u g) e v ->
-        check g (EFun x u e) (TFun u v)
-    | check_app : forall (e1 e2 : expr) (u v : type),
-        check g e1 (TFun u v) ->
-        check g e2 u ->
-        check g (EApp e1 e2) v
-    | check_rec : forall (es : fields expr) (ts : fields type),
-        nodupfs es -> nodupfs ts ->
-        relfs (check g) es ts ->
-        check g (ERec es) (TRec ts)
-    | check_prj : forall (e : expr) (x : id) (t : type) (ts : fields type),
-        In (x,t) ts ->
-        check g e (TRec ts) ->
-        check g (EPrj e x) t.
-
-(* Insufficient for records. *)
-Check check_ind.
-
-Section CheckInduction.
-    Variable P : @gamma type -> expr -> type -> Prop.
-
-    Hypothesis HSubsume : 
-        forall (g : gamma) (e : expr) (u v : type),
-        subtype u v -> check g e u -> P g e u -> P g e v.
-
-    Hypothesis HUnit : 
-        forall (g : gamma), P g EUnit TUnit.
-
-    Hypothesis HVar :
-        forall (g : gamma) (x : id) (t : type),
-        g x = Some t -> 
-        P g (EVar x) t.
-
-    Hypothesis HFun :
-        forall (g : gamma) (x : id) (u v : type) (e : expr),
-        check (bind x u g) e v ->
-        P (bind x u g) e v ->
-        P g (EFun x u e) (TFun u v).
-
-    Hypothesis HApp :
-        forall (g : gamma) (e1 e2 : expr) (u v : type),
-        check g e1 (TFun u v) ->
-        P g e1 (TFun u v) ->
-        check g e2 u ->
-        P g e2 u ->
-        P g (EApp e1 e2) v.
-
-    Hypothesis HRec :
-        forall (g : gamma) (es : fields expr) (ts : fields type),
-        nodupfs es -> nodupfs ts ->
-        relfs (check g) es ts ->
-        relfs (P g) es ts ->
-        P g (ERec es) (TRec ts).
-
-    Hypothesis HPrj :
-        forall (g : gamma) (e : expr) (x : id) (t : type) (ts : fields type),
-        In (x,t) ts ->
-        check g e (TRec ts) ->
-        P g e (TRec ts) ->
-        P g (EPrj e x) t.
-
-    Fixpoint IHCheck (g : gamma) (e : expr) (t : type) (HC :check g e t) : P g e t :=
-        match HC in check _ e' t' return (P g e' t') with
-        | check_subsume _ e u v HSuv HCeu => 
-            HSubsume g e u v HSuv HCeu (IHCheck g e u HCeu)
-        | check_unit _ => HUnit g
-        | check_var _ x t HB => HVar g x t HB
-        | check_fun _ x u v e HCev =>
-            HFun g x u v e HCev (IHCheck (bind x u g) e v HCev)
-        | check_app _ e1 e2 u v HCe1uv HCe2u =>
-            HApp g e1 e2 u v 
-                HCe1uv (IHCheck g e1 (TFun u v) HCe1uv)
-                HCe2u (IHCheck g e2 u HCe2u)
-        | check_rec _ es ts NDes NDts HRs =>
-            let fix rec_help {es' : fields expr} {ts' : fields type}
-                (HRs' : relfs (check g) es' ts') : Forall2 (relf (P g)) es' ts' :=
-                match HRs' in (Forall2 _ le lt) 
-                    return (Forall2 (relf (P g)) le lt) with
-                | Forall2_nil _ => Forall2_nil (relf (P g))
-                | Forall2_cons e t Het Hests =>
-                    Forall2_cons
-                        e t (relf_pred (IHCheck g) Het) 
-                        (rec_help Hests)
-                end in
-            HRec g es ts NDes NDts HRs (rec_help HRs)
-        | check_prj _ e x t ts Hints HCets =>
-            HPrj g e x t ts Hints HCets (IHCheck g e (TRec ts) HCets)
-        end.
-End CheckInduction.
-
-Definition checks : expr -> type -> Prop := check empty.
-
-Example benjy : 
-    checks 
-        (EApp 
-            (EFun "r" (TRec [("x",TUnit)]) 
-                (EPrj (EVar "r") "x")) 
-            (ERec [("x",EUnit);("y",EUnit)]))
-        TUnit.
-Proof.
-    apply check_app with (u := TRec [("x",TUnit)]).
-    - apply check_fun. apply check_prj with 
-        (ts := [("x",TUnit)]);
-        constructor; reflexivity.
-    - apply check_subsume with 
-        (u := TRec [("x", TUnit);("y",TUnit)]).
-        + apply st_rec_width with
-            (us := [("x",TUnit)])
-            (vs := [("y",TUnit)]).
-        + apply check_rec.
-            { constructor; try constructor;
-                try constructor; 
-                try intros DUMB; inv DUMB;
-                try discriminate. inv H. }
-            { constructor; try constructor;
-                try constructor; 
-                try intros DUMB; inv DUMB;
-                try discriminate. inv H. }
-            { constructor.
-                - split; try reflexivity. constructor. 
-                - constructor.
-                    + split.
-                        * reflexivity.
-                        * constructor.
-                    + constructor. }
-Qed. 
-
-(* Values *)
-Inductive value : expr -> Prop :=
-    | value_unit : value EUnit
-    | value_fun : forall (x : id) (t : type) (e : expr),
-        value (EFun x t e)
-    | value_rec : forall (vs : fields expr),
-        predfs value vs ->
-        value (ERec vs).
-
-Section ValueDec.
-    Fixpoint value_dec (v : expr) : {value v} + {~ value v}. 
-    Proof.
-        destruct v.
-        - left. constructor.
-        - right. intros HF. inv HF.
-        - left. constructor.
-        - right. intros HF. inv HF.
-        - induction fs.
-            + left. constructor. constructor.
-            + destruct (value_dec (snd a)) as [AV | AV].
-                { destruct IHfs as [V | V].
-                    - pose proof 
-                        (fun x : field expr => value_dec (snd x)) as PFV.
-                        pose proof @Forall_dec
-                            (field expr) (predf value) 
-                            PFV fs as FD.
-                        destruct FD as [FV | FV].
-                        + left. constructor. 
-                            constructor; assumption.
-                        + right. intros HF. apply FV.
-                            inv HF. inv H0. assumption.
-                    - right. intros HF. apply V. 
-                        inv HF. inv H0. constructor.
-                        assumption. }
-                { right. intros HF. apply AV. inv HF.
-                    inv H0. assumption. }
-        - right. intros HF. inv HF.
-    Qed.
-End ValueDec.
-
-(* free variables *)
-Fixpoint fv (e : expr) : IS.t :=
-    match e with
-    | EUnit => IS.empty
-    | EVar x => IS.singleton x
-    | EFun x _ e => IS.remove x (fv e)
-    | EApp e1 e2 => IS.union (fv e1) (fv e2)
-    | ERec (es) => 
-        fold_right 
-            (fun (e : field expr) acc => 
-                IS.union acc (fv (snd e)))
-            IS.empty es
-    | EPrj e _ => fv e
-    end.
-
-(* Capture-avoiding Substitution *)
-Inductive sub (x : id) (es : expr) : expr -> expr -> Prop :=
-    | sub_unit : sub x es EUnit EUnit
-    | sub_hit : sub x es (EVar x) es
-    | sub_miss : forall (y : id), 
-        x <> y -> 
-        sub x es (EVar y) (EVar y)
-    | sub_fun_bound : forall (t : type) (e : expr),
-        sub x es (EFun x t e) (EFun x t e)
-    | sub_fun_notfree : forall (y : string) (t : type) (e e' : expr),
-        x <> y ->
-        ~ IS.In y (fv es) -> 
-        sub x es e e' -> 
-        sub x es (EFun y t e) (EFun y t e')
-    | sub_fun_free : forall (y z : id) (t : type) (e e' e'' : expr),
-        x <> y -> 
-        x <> z -> 
-        y <> z ->
-        IS.In y (fv es) -> 
-        ~ IS.In z (fv es) ->
-        ~ IS.In z (fv e) ->
-        sub y (EVar z) e e' -> 
-        sub x es e' e'' -> 
-        sub x es (EFun y t e) (EFun z t e'')
-    | sub_app : forall (e1 e1' e2 e2' : expr),
-        sub x es e1 e1' -> 
-        sub x es e2 e2' -> 
-        sub x es (EApp e1 e2) (EApp e1' e2')
-    | sub_rec : forall (fs fs' : fields expr),
-        relfs (sub x es) fs fs' ->
-        sub x es (ERec fs) (ERec fs')
-    | sub_prj : forall (e e' : expr) (y : id),
-        sub x es e e' ->
-        sub x es (EPrj e y) (EPrj e' y).
-
-Check sub_ind.
-
-Section SubstitutionInduction.
-    Variable P : id -> expr -> expr -> expr -> Prop.
-
-    Hypothesis HUnit : 
-        forall (x : id) (es : expr), 
-        P x es EUnit EUnit.
-
-    Hypothesis HHit : 
-        forall (x : id) (es : expr),
-        P x es (EVar x) es.
-
-    Hypothesis HMiss : 
-        forall (x : id) (es : expr) (y : id),
-        x <> y -> P x es (EVar y) (EVar y).
-
-    Hypothesis HFunBound : 
-        forall (x : id) (es : expr) (t : type) (e : expr),
-        P x es (EFun x t e) (EFun x t e).
-
-    Hypothesis HFunNotFree : 
-        forall (x : id) (es : expr) (y : string) (t : type) (e e' : expr),
-        x <> y -> ~ IS.In y (fv es) ->
-        sub x es e e' -> P x es e e' -> 
-        P x es (EFun y t e) (EFun y t e').
-
-    Hypothesis HFunFree :
-        forall (x : id) (es : expr) (y z : id)
-        (t : type) (e e' e'' : expr),
-        x <> y -> x <> z ->
-        y <> z -> IS.In y (fv es) ->
-        ~ IS.In z (fv es) -> ~ IS.In z (fv e) ->
-        sub y (EVar z) e e' -> P y (EVar z) e e' ->
-        sub x es e' e'' -> P x es e' e'' -> 
-        P x es (EFun y t e) (EFun z t e'').
-
-    Hypothesis HApp :
-        forall (x : id) (es e1 e1' e2 e2' : expr),
-        sub x es e1 e1' -> P x es e1 e1' ->
-        sub x es e2 e2' -> P x es e2 e2' -> 
-        P x es (EApp e1 e2) (EApp e1' e2').
-
-    Hypothesis HRec : 
-        forall (x : id) (es : expr) (fs fs' : fields expr),
-        relfs (sub x es) fs fs' -> 
-        relfs (P x es) fs fs' ->
-        P x es (ERec fs) (ERec fs').
-
-    Hypothesis HPrj :
-        forall (x : id) (es e e' : expr) (y : id),
-        sub x es e e' -> P x es e e' -> 
-        P x es (EPrj e y) (EPrj e' y).
-
-    Fixpoint IHSubstitute (x : id) (es e e' : expr)
-    (HS : sub x es e e') {struct HS} : P x es e e' :=
-        match HS in sub _ _ pe pe' return P x es pe pe' with
-        | sub_unit _ _ => HUnit x es
-        | sub_hit _ _ => HHit x es
-        | sub_miss _ _ y Hxy => HMiss x es y Hxy
-        | sub_fun_bound _ _ t e => HFunBound x es t e
-        | sub_fun_notfree _ _ y t e e' Hxy Hines HS =>
-            HFunNotFree x es y t e e' 
-                Hxy Hines HS (IHSubstitute x es e e' HS)
-        | sub_fun_free _ _ y z t e e' e'' 
-            Hxy Hxz Hyz Hinyes Hinzes Hinze HSee' HSe'e'' =>
-            HFunFree x es y z t e e' e'' 
-                Hxy Hxz Hyz Hinyes Hinzes Hinze
-                HSee' (IHSubstitute y (EVar z) e e' HSee')
-                HSe'e'' (IHSubstitute x es e' e'' HSe'e'')
-        | sub_app _ _ e1 e1' e2 e2' HS1 HS2 =>
-            HApp x es e1 e1' e2 e2'
-                HS1 (IHSubstitute x es e1 e1' HS1)
-                HS2 (IHSubstitute x es e2 e2' HS2)
-        | sub_rec _ _ fs fs' HRs =>
-            let fix rec_help {fds : fields expr} {fds' : fields expr}
-            (HRs' : relfs (sub x es) fds fds') : Forall2 (relf (P x es)) fds fds' :=
-                match HRs' in (Forall2 _ l l') 
-                    return (Forall2 (relf (P x es)) l l') with
-                | Forall2_nil _ => Forall2_nil (relf (P x es))
-                | Forall2_cons fd fd' HRhead HRtail =>
-                    Forall2_cons
-                        fd fd' (relf_pred (IHSubstitute x es) HRhead) 
-                        (rec_help HRtail)
-                end in
-            HRec x es fs fs' HRs (rec_help HRs)
-        | sub_prj _ _ e e' y HS =>
-            HPrj x es e e' y HS (IHSubstitute x es e e' HS)
-        end.
-End SubstitutionInduction.
-
-Axiom sub_exists : forall (x : id) (s e : expr), exists e', sub x s e e'.
-
-(* Dynamic Semantics *)
-Inductive step : expr -> expr -> Prop :=
-    | step_redux : forall (x : id) (t : type) (e es e' : expr),
-        sub x es e e' ->
-        step (EApp (EFun x t e) es) e'
-    | step_app : forall (e1 e2 e1' : expr),
-        step e1 e1' ->
-        step (EApp e1 e2) (EApp e1' e2)
-    | step_prj_rec : forall (es : fields expr) (x : id) (e : expr),
-        In (x,e) es ->
-        step (EPrj (ERec es) x) e
-    | step_prj : forall (e e' : expr) (x : id),
-        step e e' ->
-        step (EPrj e x) (EPrj e' x)
-    | step_rec : forall (vs es : fields expr) (x : id) (e e' : expr),
-        predfs value vs ->
-        step e e' ->
-        step (ERec (vs ++ (x,e) :: es)) (ERec (vs ++ (x,e') :: es)).
-
-Check step_ind.
-
-(* Inversion on Subsumption. *)
-Section InvSubsumption.
-    Lemma inv_top :
-        forall (t : type),
-        subtype TTop t -> t = TTop.
-    Proof.
-        intros t HS. dependent induction HS; auto.
-    Qed.
-            
-    Lemma inv_unit :
-        forall (t : type),
-        subtype t TUnit -> t = TUnit.
-    Proof.
-        intros t HS. dependent induction HS; auto.
+    Module SSType.
+        Inductive type : Type :=
+            | TTop
+            | TUnit
+            | TFun (t t' : type)
+            | TRec (fs : fields type).
+
+        Definition fields_type := fields type.
+
+        (* Doesn't work because Coq's Scheme Command is stupid :
+            To use Scheme the Types must be mutually defined 
+            with the "with" keyword. *)
+        Fail Scheme type_rec' := Induction for type Sort Type
+            with fields_type_rec := Induction for fields_type Sort Type.
+
+        (* custom induction principle for Type type *)
+        Section TypeInduction.
+            Variable P : type -> Prop.
+
+            Hypothesis HTop : P TTop.
+
+            Hypothesis HUnit : P TUnit.
+
+            Hypothesis HFun : forall (t t' : type),
+                P t -> P t' -> P (TFun t t').
+
+            Hypothesis HRec : forall (fs : fields type),
+                predfs P fs -> P (TRec fs).
+
+            Fixpoint IHType (t : type) : P t :=
+                match t as ty return P ty with 
+                | TTop => HTop
+                | TUnit => HUnit
+                | TFun t1 t2 => HFun t1 t2 (IHType t1) (IHType t2)
+                | TRec fs =>
+                    let fix list_ih (fs' : fields type) : predfs P fs' :=
+                        match fs' as fs_ty return predfs P fs_ty with
+                        | [] => Forall_nil (predf P)
+                        | hf :: tf => Forall_cons hf (IHType (snd hf)) (list_ih tf)
+                        end in
+                    HRec fs (list_ih fs)
+                end.
+        End TypeInduction.
+
+        Ltac indtype t := induction t using IHType.
+    End SSType.
+    Export SSType.
+
+    (* The Subtyping Relation *)
+    Inductive subtype : type -> type -> Prop :=
+        | st_refl : forall (t : type), 
+            subtype t t
+        | st_trans : forall (t u v : type),
+            subtype t u -> 
+            subtype u v ->
+            subtype t v
+        | st_top : forall (t : type),
+            subtype t TTop
+        | st_fun : forall (u u' v v' : type),
+            subtype u' u ->
+            subtype v v' ->
+            subtype (TFun u v) (TFun u' v')
+        | st_rec_width : forall (us vs : fields type),
+            subtype (TRec (us ++ vs)) (TRec us)
+        | st_rec_depth : forall (us vs : fields type),
+            relfs subtype us vs ->
+            subtype (TRec us) (TRec vs)
+        | st_rec_perm : forall (us vs : fields type),
+            perm us vs ->
+            subtype (TRec us) (TRec vs).
+
+    Check subtype_ind.
+    Compute subtype_ind.
+
+    Section SubtypeInduction.
+        Variable P : type -> type -> Prop.
+
+        Hypothesis HRefl : forall (t : type), P t t.
+
+        Hypothesis HTrans : forall (t u v : type),
+            subtype t u -> P t u ->
+            subtype u v -> P u v -> P t v.
+
+        Hypothesis HTop : forall (t : type), P t TTop.
+
+        Hypothesis HFun : forall (u u' v v' : type),
+            subtype u' u -> P u' u ->
+            subtype v v' -> P v v' ->
+            P (TFun u v) (TFun u' v').
+
+        Hypothesis HRecWidth : forall (us vs : fields type),
+            P (TRec (us ++ vs)) (TRec us).
+
+        Hypothesis HRecDepth : forall (us vs : fields type),
+            relfs subtype us vs -> relfs P us vs ->
+            P (TRec us) (TRec vs).
+
+        Hypothesis HRecPerm : forall (us vs : fields type),
+            perm us vs -> P (TRec us) (TRec vs).
+        
+        Fixpoint IHSubtype (t t' : type) (HS : subtype t t') {struct HS} : P t t' :=
+            match HS in (subtype w w') return (P w w') with
+            | st_refl t => HRefl t
+            | st_trans t u v Htu Huv =>
+                HTrans t u v Htu (IHSubtype t u Htu) Huv (IHSubtype u v Huv)
+            | st_top t => HTop t
+            | st_fun u u' v v' Hu Hv =>
+                HFun u u' v v' Hu (IHSubtype u' u Hu) Hv (IHSubtype v v' Hv)
+            | st_rec_width us vs => HRecWidth us vs
+            | st_rec_depth us vs HRs =>
+                let fix depth_helper {us' : fields type} {vs' : fields type}
+                    (HRs' : relfs subtype us' vs') : Forall2 (relf P) us' vs' :=
+                    match HRs' in (Forall2 _ lu lv) 
+                        return (Forall2 (relf P) lu lv) with
+                    | Forall2_nil _ => Forall2_nil (relf P)
+                    | Forall2_cons u v Huv Husvs =>
+                        Forall2_cons
+                            u v (relf_pred IHSubtype Huv) 
+                            (depth_helper Husvs)
+                    end in
+                HRecDepth us vs HRs (depth_helper HRs) 
+            | st_rec_perm us vs HP => HRecPerm us vs HP
+            end.
+    End SubtypeInduction.
+
+    Lemma st_fields_refl :
+        forall (fs : fields type), relfs subtype fs fs.
+    Proof. induction fs; constructor.
+        - split; constructor.
+        - assumption.
     Qed.
 
-    Lemma inv_fun :
-        forall (t a b : type),
-        subtype t (TFun a b) ->
-        exists (a' b' : type),
-        t = TFun a' b' /\ subtype a a' /\ subtype b' b.
+    Lemma st_fields_rec :
+        forall (us vs : fields type),
+        relfs subtype us vs -> subtype (TRec us) (TRec vs).
     Proof.
-        intros t a b HS.
-        dependent induction HS.
-        - exists a. exists b. split.
-            + reflexivity.
-            + split; constructor.
-        - specialize IHHS2 with 
-            (a0 := a) (b0 := b).
-            assert (HR : TFun a b = TFun a b);
-            try reflexivity.
-            apply IHHS2 in HR as [a' [b' [HU [HSA HSB]]]].
-            apply IHHS1 in HU as [a'' [b'' [HT [HSA' HSB']]]].
-            exists a''. exists b''. split.
-            + assumption.
-            + split.
-                * apply st_trans with
-                    (t := a) (u := a') (v := a'');
-                    assumption.
-                * apply st_trans with
-                    (t := b'') (u := b') (v := b);
-                assumption.
-        - exists u. exists v. split.
-            + reflexivity.
-            + split; assumption.
+        intros us vs HS. constructor. assumption.
     Qed.
 
-    Lemma inv_rec :
-        forall (t : type) (ts : fields type),
-        subtype t (TRec ts) ->
-        exists (us : fields type),
-        t = TRec us /\ subtype (TRec us) (TRec ts).
+    Example record_subtyping_makes_sense :
+        subtype 
+            (TRec [("x",TUnit);("y",TUnit)]) 
+            (TRec [("y",TTop)]).
     Proof.
-        intros t ts HS. dependent induction HS.
-        - exists ts. split; auto.
-            apply st_refl.
-        - specialize IHHS2 with (ts0 := ts).
-            assert (HRts : TRec ts = TRec ts);
-            try reflexivity.
-            apply IHHS2 in HRts as IH2.
-            destruct IH2 as [us [HU HSusts]].
-            specialize IHHS1 with (ts := us).
-            apply IHHS1 in HU as IH1.
-            destruct IH1 as [vs [HT HSvsus]].
-            exists vs. split; auto.
-            apply st_trans with 
-                (t := (TRec vs)) (u := TRec us) (v := TRec ts);
-            assumption.
-        - exists (ts ++ vs). split; constructor.
-        - exists us. split; constructor. assumption.
-        - exists us. split; auto.
-            apply st_rec_perm. assumption.
-    Qed.
-End InvSubsumption.
-
-Section CanonicalForms.
-    Definition canon_unit (v : expr) : Prop :=
-        value v -> checks v TUnit -> v = EUnit.
-
-    Definition canon_fun (v : expr) : Prop :=
-        forall (a b : type),
-        value v -> checks v (TFun a b) -> 
-        exists (x : id) (t : type) (e : expr), 
-        subtype a t /\ v = EFun x t e.
-
-    Definition canon_rec (v : expr) := 
-        forall (ts : fields type),
-        value v -> checks v (TRec ts) ->
-        exists (es : fields expr) (us : fields type), 
-        v = ERec es /\
-        relfs (check empty) es us /\ 
-        subtype (TRec us) (TRec ts).
-
-    Lemma canonical_forms_unit : 
-        forall (v : expr), canon_unit v.
-    Proof.
-        unfold canon_unit. intros v HV HChk;
-        dependent induction HChk.
-        - apply inv_unit in H as HU. auto.
-        - reflexivity.
-        - inversion HV.
-        - inversion HV.
-        - inversion HV.
+        apply st_trans with (u := TRec [("y",TUnit)]).
+        - apply st_trans with (u := TRec [("y", TUnit); ("x", TUnit)]).
+            + apply st_rec_perm. constructor.
+            + assert (HE : [("y", TUnit); ("x", TUnit)] 
+                = [("y", TUnit)] ++ [("x", TUnit)]);
+                try reflexivity. rewrite HE.
+                apply st_rec_width.
+        - apply st_rec_depth. constructor.
+            + split; auto. apply st_top.
+            + constructor.
     Qed.
 
-    Lemma canonical_forms_fun :
-        forall (v : expr), canon_fun v.
-    Proof.
-        unfold canon_fun. intros v t t' HV HChk.
-        dependent induction HChk.
-        - apply inv_fun in H as HU.
-            destruct HU as [a' [b' [HF [HSA HSB]]]].
-            specialize IHHChk with
-                (t := a') (t' := b').
-            pose proof (IHHChk HV HF) as IH.
-            destruct IH as [x [w [e' [HSW HFW]]]].
-            exists x. exists w. exists e'. split.
-            + apply st_trans with
-                (t := t) (u := a') (v := w);
-                assumption.
-            + assumption.
-        - inversion HV.
-        - exists x. exists t. exists e. 
-            split; constructor.
-        - inversion HV.
-        - inversion HV.
-    Qed.
+    Module SSExpr.
+        Inductive expr : Type :=
+            | EUnit
+            | EVar (x : id)
+            | EFun (x : id) (t : type) (e : expr)
+            | EApp (e1 e2 : expr)
+            | ERec (fs : fields expr)
+            | EPrj (e : expr) (x : id).
 
-    Lemma canonical_forms_rec :
-        forall (v : expr), canon_rec v.
-    Proof.
-        unfold canon_rec. intros v ts HV HChk.
-        dependent induction HChk.
-        - apply inv_rec in H as [us [HU HSusts]].
-            specialize IHHChk with (ts := us).
-            apply IHHChk in HV as IH; auto.
-            destruct IH as [es [vs [Hrec [HR HSvsus]]]].
-            exists es. exists vs. split; auto. split; auto.
-            apply st_trans with
-                (t := (TRec vs)) (u := (TRec us)) (v := (TRec ts));
-            assumption.
-        - inv HV.
-        - inv HV.
-        - exists es. exists ts. 
-            split; try reflexivity.
-            induction HV; subst; constructor;
-            try assumption;
-            try apply st_refl.
-        - inv HV. 
-    Qed.
-End CanonicalForms.
+        (* custom induction principle for Type expr *)
+        Section ExprInduction.
+            Variable P : expr -> Prop.
 
-Section Progress.
-    Lemma st_fields_name :
-        forall (us ws : fields type),
-        subtype (TRec us) (TRec ws) ->
-        forall (x : id) (w : type),
-        In (x,w) ws ->
-        exists (u : type),
-        In (x,u) us /\ subtype u w.
+            Hypothesis HUnit : P EUnit.
+
+            Hypothesis HVar : forall (x : id), P (EVar x).
+
+            Hypothesis HFun : forall (x : id) (t : type) (e : expr),
+                P e -> P (EFun x t e).
+
+            Hypothesis HApp : forall (e1 e2 : expr),
+                P e1 -> P e2 -> P (EApp e1 e2).
+
+            Hypothesis HRec : forall (fs : fields expr),
+                predfs P fs -> P (ERec fs).
+
+            Hypothesis HPrj : forall (e : expr) (x : id),
+                P e -> P (EPrj e x).
+
+            Check Forall_cons.
+
+            Fixpoint IHExpr (e : expr) : P e :=
+                match e as ee return (P ee) with
+                | EUnit => HUnit
+                | EVar x => HVar x
+                | EFun x t e => HFun x t e (IHExpr e)
+                | EApp e1 e2 => HApp e1 e2 (IHExpr e1) (IHExpr e2)
+                | ERec fs =>
+                    let fix rec_help (fs' : fields expr) : predfs P fs' :=
+                        match fs' as fs'' return (predfs P fs'') with
+                        | [] => Forall_nil (predf P)
+                        | hf::tf => Forall_cons hf (IHExpr (snd hf)) (rec_help tf)
+                        end in
+                    HRec fs (rec_help fs)
+                | EPrj e x => HPrj e x (IHExpr e)
+                end.
+        End ExprInduction.
+
+        Ltac indexpr e := induction e using IHExpr.
+    End SSExpr.
+    Export SSExpr.
+
+    (* Static Semantics with Subsumption *)
+    Inductive check (g : gamma) : expr -> type -> Prop :=
+        | check_subsume : forall (e : expr) (u v : type),
+            subtype u v ->
+            check g e u ->
+            check g e v
+        | check_unit :
+            check g EUnit TUnit
+        | check_var : forall (x : id) (t : type),
+            g x = Some t ->
+            check g (EVar x) t
+        | check_fun : forall (x : id) (u v : type) (e : expr),
+            check (bind x u g) e v ->
+            check g (EFun x u e) (TFun u v)
+        | check_app : forall (e1 e2 : expr) (u v : type),
+            check g e1 (TFun u v) ->
+            check g e2 u ->
+            check g (EApp e1 e2) v
+        | check_rec : forall (es : fields expr) (ts : fields type),
+            nodupfs es -> nodupfs ts ->
+            relfs (check g) es ts ->
+            check g (ERec es) (TRec ts)
+        | check_prj : forall (e : expr) (x : id) (t : type) (ts : fields type),
+            In (x,t) ts ->
+            check g e (TRec ts) ->
+            check g (EPrj e x) t.
+
+    (* Insufficient for records. *)
+    Check check_ind.
+
+    Section CheckInduction.
+        Variable P : @gamma type -> expr -> type -> Prop.
+
+        Hypothesis HSubsume : 
+            forall (g : gamma) (e : expr) (u v : type),
+            subtype u v -> check g e u -> P g e u -> P g e v.
+
+        Hypothesis HUnit : 
+            forall (g : gamma), P g EUnit TUnit.
+
+        Hypothesis HVar :
+            forall (g : gamma) (x : id) (t : type),
+            g x = Some t -> 
+            P g (EVar x) t.
+
+        Hypothesis HFun :
+            forall (g : gamma) (x : id) (u v : type) (e : expr),
+            check (bind x u g) e v ->
+            P (bind x u g) e v ->
+            P g (EFun x u e) (TFun u v).
+
+        Hypothesis HApp :
+            forall (g : gamma) (e1 e2 : expr) (u v : type),
+            check g e1 (TFun u v) ->
+            P g e1 (TFun u v) ->
+            check g e2 u ->
+            P g e2 u ->
+            P g (EApp e1 e2) v.
+
+        Hypothesis HRec :
+            forall (g : gamma) (es : fields expr) (ts : fields type),
+            nodupfs es -> nodupfs ts ->
+            relfs (check g) es ts ->
+            relfs (P g) es ts ->
+            P g (ERec es) (TRec ts).
+
+        Hypothesis HPrj :
+            forall (g : gamma) (e : expr) (x : id) (t : type) (ts : fields type),
+            In (x,t) ts ->
+            check g e (TRec ts) ->
+            P g e (TRec ts) ->
+            P g (EPrj e x) t.
+
+        Fixpoint IHCheck (g : gamma) (e : expr) (t : type) (HC :check g e t) : P g e t :=
+            match HC in check _ e' t' return (P g e' t') with
+            | check_subsume _ e u v HSuv HCeu => 
+                HSubsume g e u v HSuv HCeu (IHCheck g e u HCeu)
+            | check_unit _ => HUnit g
+            | check_var _ x t HB => HVar g x t HB
+            | check_fun _ x u v e HCev =>
+                HFun g x u v e HCev (IHCheck (bind x u g) e v HCev)
+            | check_app _ e1 e2 u v HCe1uv HCe2u =>
+                HApp g e1 e2 u v 
+                    HCe1uv (IHCheck g e1 (TFun u v) HCe1uv)
+                    HCe2u (IHCheck g e2 u HCe2u)
+            | check_rec _ es ts NDes NDts HRs =>
+                let fix rec_help {es' : fields expr} {ts' : fields type}
+                    (HRs' : relfs (check g) es' ts') : Forall2 (relf (P g)) es' ts' :=
+                    match HRs' in (Forall2 _ le lt) 
+                        return (Forall2 (relf (P g)) le lt) with
+                    | Forall2_nil _ => Forall2_nil (relf (P g))
+                    | Forall2_cons e t Het Hests =>
+                        Forall2_cons
+                            e t (relf_pred (IHCheck g) Het) 
+                            (rec_help Hests)
+                    end in
+                HRec g es ts NDes NDts HRs (rec_help HRs)
+            | check_prj _ e x t ts Hints HCets =>
+                HPrj g e x t ts Hints HCets (IHCheck g e (TRec ts) HCets)
+            end.
+    End CheckInduction.
+
+    Definition checks : expr -> type -> Prop := check empty.
+
+    Example benjy : 
+        checks 
+            (EApp 
+                (EFun "r" (TRec [("x",TUnit)]) 
+                    (EPrj (EVar "r") "x")) 
+                (ERec [("x",EUnit);("y",EUnit)]))
+            TUnit.
     Proof.
-        intros us ws HS.
-        dependent induction HS using IHSubtype; intros x w Hinws.
-        - subst. exists w. 
-            split; auto. constructor.
-        - assert (HSusws : subtype (TRec us) (TRec ws)).
-            + apply st_trans with (u := u); assumption.
-            + pose proof inv_rec u ws HS2 as [vs [Huvs HSvws]]. subst.
-                assert (Hduhu : TRec us = TRec us);
-                assert (Hduhv : TRec vs = TRec vs);
-                assert (Hduhw : TRec ws = TRec ws);
+        apply check_app with (u := TRec [("x",TUnit)]).
+        - apply check_fun. apply check_prj with 
+            (ts := [("x",TUnit)]);
+            constructor; reflexivity.
+        - apply check_subsume with 
+            (u := TRec [("x", TUnit);("y",TUnit)]).
+            + apply st_rec_width with
+                (us := [("x",TUnit)])
+                (vs := [("y",TUnit)]).
+            + apply check_rec.
+                { constructor; try constructor;
+                    try constructor; 
+                    try intros DUMB; inv DUMB;
+                    try discriminate. inv H. }
+                { constructor; try constructor;
+                    try constructor; 
+                    try intros DUMB; inv DUMB;
+                    try discriminate. inv H. }
+                { constructor.
+                    - split; try reflexivity. constructor. 
+                    - constructor.
+                        + split.
+                            * reflexivity.
+                            * constructor.
+                        + constructor. }
+    Qed. 
+
+    (* Values *)
+    Module Value.
+        Inductive value : expr -> Prop :=
+            | value_unit : value EUnit
+            | value_fun : forall (x : id) (t : type) (e : expr),
+                value (EFun x t e)
+            | value_rec : forall (vs : fields expr),
+                predfs value vs ->
+                value (ERec vs).
+
+        Section ValueDec.
+            Fixpoint value_dec (v : expr) : {value v} + {~ value v}. 
+            Proof.
+                destruct v.
+                - left. constructor.
+                - right. intros HF. inv HF.
+                - left. constructor.
+                - right. intros HF. inv HF.
+                - induction fs.
+                    + left. constructor. constructor.
+                    + destruct (value_dec (snd a)) as [AV | AV].
+                        { destruct IHfs as [V | V].
+                            - pose proof 
+                                (fun x : field expr => value_dec (snd x)) as PFV.
+                                pose proof @Forall_dec
+                                    (field expr) (predf value) 
+                                    PFV fs as FD.
+                                destruct FD as [FV | FV].
+                                + left. constructor. 
+                                    constructor; assumption.
+                                + right. intros HF. apply FV.
+                                    inv HF. inv H0. assumption.
+                            - right. intros HF. apply V. 
+                                inv HF. inv H0. constructor.
+                                assumption. }
+                        { right. intros HF. apply AV. inv HF.
+                            inv H0. assumption. }
+                - right. intros HF. inv HF.
+            Qed.
+        End ValueDec.
+    End Value.
+    Export Value.
+
+    Module Step.
+        (* free variables *)
+        Fixpoint fv (e : expr) : IS.t :=
+            match e with
+            | EUnit => IS.empty
+            | EVar x => IS.singleton x
+            | EFun x _ e => IS.remove x (fv e)
+            | EApp e1 e2 => IS.union (fv e1) (fv e2)
+            | ERec (es) => 
+                fold_right 
+                    (fun (e : field expr) acc => 
+                        IS.union acc (fv (snd e)))
+                    IS.empty es
+            | EPrj e _ => fv e
+            end.
+
+        (* Capture-avoiding Substitution *)
+        Inductive sub (x : id) (es : expr) : expr -> expr -> Prop :=
+            | sub_unit : sub x es EUnit EUnit
+            | sub_hit : sub x es (EVar x) es
+            | sub_miss : forall (y : id), 
+                x <> y -> 
+                sub x es (EVar y) (EVar y)
+            | sub_fun_bound : forall (t : type) (e : expr),
+                sub x es (EFun x t e) (EFun x t e)
+            | sub_fun_notfree : forall (y : string) (t : type) (e e' : expr),
+                x <> y ->
+                ~ IS.In y (fv es) -> 
+                sub x es e e' -> 
+                sub x es (EFun y t e) (EFun y t e')
+            | sub_fun_free : forall (y z : id) (t : type) (e e' e'' : expr),
+                x <> y -> 
+                x <> z -> 
+                y <> z ->
+                IS.In y (fv es) -> 
+                ~ IS.In z (fv es) ->
+                ~ IS.In z (fv e) ->
+                sub y (EVar z) e e' -> 
+                sub x es e' e'' -> 
+                sub x es (EFun y t e) (EFun z t e'')
+            | sub_app : forall (e1 e1' e2 e2' : expr),
+                sub x es e1 e1' -> 
+                sub x es e2 e2' -> 
+                sub x es (EApp e1 e2) (EApp e1' e2')
+            | sub_rec : forall (fs fs' : fields expr),
+                relfs (sub x es) fs fs' ->
+                sub x es (ERec fs) (ERec fs')
+            | sub_prj : forall (e e' : expr) (y : id),
+                sub x es e e' ->
+                sub x es (EPrj e y) (EPrj e' y).
+
+        Section SubstitutionInduction.
+            Variable P : id -> expr -> expr -> expr -> Prop.
+
+            Hypothesis HUnit : 
+                forall (x : id) (es : expr), 
+                P x es EUnit EUnit.
+
+            Hypothesis HHit : 
+                forall (x : id) (es : expr),
+                P x es (EVar x) es.
+
+            Hypothesis HMiss : 
+                forall (x : id) (es : expr) (y : id),
+                x <> y -> P x es (EVar y) (EVar y).
+
+            Hypothesis HFunBound : 
+                forall (x : id) (es : expr) (t : type) (e : expr),
+                P x es (EFun x t e) (EFun x t e).
+
+            Hypothesis HFunNotFree : 
+                forall (x : id) (es : expr) (y : string) (t : type) (e e' : expr),
+                x <> y -> ~ IS.In y (fv es) ->
+                sub x es e e' -> P x es e e' -> 
+                P x es (EFun y t e) (EFun y t e').
+
+            Hypothesis HFunFree :
+                forall (x : id) (es : expr) (y z : id)
+                (t : type) (e e' e'' : expr),
+                x <> y -> x <> z ->
+                y <> z -> IS.In y (fv es) ->
+                ~ IS.In z (fv es) -> ~ IS.In z (fv e) ->
+                sub y (EVar z) e e' -> P y (EVar z) e e' ->
+                sub x es e' e'' -> P x es e' e'' -> 
+                P x es (EFun y t e) (EFun z t e'').
+
+            Hypothesis HApp :
+                forall (x : id) (es e1 e1' e2 e2' : expr),
+                sub x es e1 e1' -> P x es e1 e1' ->
+                sub x es e2 e2' -> P x es e2 e2' -> 
+                P x es (EApp e1 e2) (EApp e1' e2').
+
+            Hypothesis HRec : 
+                forall (x : id) (es : expr) (fs fs' : fields expr),
+                relfs (sub x es) fs fs' -> 
+                relfs (P x es) fs fs' ->
+                P x es (ERec fs) (ERec fs').
+
+            Hypothesis HPrj :
+                forall (x : id) (es e e' : expr) (y : id),
+                sub x es e e' -> P x es e e' -> 
+                P x es (EPrj e y) (EPrj e' y).
+
+            Fixpoint IHSubstitute (x : id) (es e e' : expr)
+            (HS : sub x es e e') {struct HS} : P x es e e' :=
+                match HS in sub _ _ pe pe' return P x es pe pe' with
+                | sub_unit _ _ => HUnit x es
+                | sub_hit _ _ => HHit x es
+                | sub_miss _ _ y Hxy => HMiss x es y Hxy
+                | sub_fun_bound _ _ t e => HFunBound x es t e
+                | sub_fun_notfree _ _ y t e e' Hxy Hines HS =>
+                    HFunNotFree x es y t e e' 
+                        Hxy Hines HS (IHSubstitute x es e e' HS)
+                | sub_fun_free _ _ y z t e e' e'' 
+                    Hxy Hxz Hyz Hinyes Hinzes Hinze HSee' HSe'e'' =>
+                    HFunFree x es y z t e e' e'' 
+                        Hxy Hxz Hyz Hinyes Hinzes Hinze
+                        HSee' (IHSubstitute y (EVar z) e e' HSee')
+                        HSe'e'' (IHSubstitute x es e' e'' HSe'e'')
+                | sub_app _ _ e1 e1' e2 e2' HS1 HS2 =>
+                    HApp x es e1 e1' e2 e2'
+                        HS1 (IHSubstitute x es e1 e1' HS1)
+                        HS2 (IHSubstitute x es e2 e2' HS2)
+                | sub_rec _ _ fs fs' HRs =>
+                    let fix rec_help {fds : fields expr} {fds' : fields expr}
+                    (HRs' : relfs (sub x es) fds fds') : Forall2 (relf (P x es)) fds fds' :=
+                        match HRs' in (Forall2 _ l l') 
+                            return (Forall2 (relf (P x es)) l l') with
+                        | Forall2_nil _ => Forall2_nil (relf (P x es))
+                        | Forall2_cons fd fd' HRhead HRtail =>
+                            Forall2_cons
+                                fd fd' (relf_pred (IHSubstitute x es) HRhead) 
+                                (rec_help HRtail)
+                        end in
+                    HRec x es fs fs' HRs (rec_help HRs)
+                | sub_prj _ _ e e' y HS =>
+                    HPrj x es e e' y HS (IHSubstitute x es e e' HS)
+                end.
+        End SubstitutionInduction.
+
+        Axiom sub_exists : forall (x : id) (s e : expr), exists e', sub x s e e'.
+
+        (* Dynamic Semantics *)
+        Inductive step : expr -> expr -> Prop :=
+            | step_redux : forall (x : id) (t : type) (e es e' : expr),
+                sub x es e e' ->
+                step (EApp (EFun x t e) es) e'
+            | step_app : forall (e1 e2 e1' : expr),
+                step e1 e1' ->
+                step (EApp e1 e2) (EApp e1' e2)
+            | step_prj_rec : forall (es : fields expr) (x : id) (e : expr),
+                In (x,e) es ->
+                step (EPrj (ERec es) x) e
+            | step_prj : forall (e e' : expr) (x : id),
+                step e e' ->
+                step (EPrj e x) (EPrj e' x)
+            | step_rec : forall (vs es : fields expr) (x : id) (e e' : expr),
+                predfs value vs ->
+                step e e' ->
+                step (ERec (vs ++ (x,e) :: es)) (ERec (vs ++ (x,e') :: es)).
+    End Step.
+    Export Step.
+
+    (* Inversion on Subsumption. *)
+    Section InvSubsumption.
+        Lemma inv_top :
+            forall (t : type),
+            subtype TTop t -> t = TTop.
+        Proof.
+            intros t HS. dependent induction HS; auto.
+        Qed.
+                
+        Lemma inv_unit :
+            forall (t : type),
+            subtype t TUnit -> t = TUnit.
+        Proof.
+            intros t HS. dependent induction HS; auto.
+        Qed.
+
+        Lemma inv_fun :
+            forall (t a b : type),
+            subtype t (TFun a b) ->
+            exists (a' b' : type),
+            t = TFun a' b' /\ subtype a a' /\ subtype b' b.
+        Proof.
+            intros t a b HS.
+            dependent induction HS.
+            - exists a. exists b. split.
+                + reflexivity.
+                + split; constructor.
+            - specialize IHHS2 with 
+                (a0 := a) (b0 := b).
+                assert (HR : TFun a b = TFun a b);
                 try reflexivity.
-                pose proof IHHS2 vs ws Hduhv Hduhw x w as IH2.
-                apply IH2 in Hinws as [w' [Hinvs HSw'w]].
-                pose proof IHHS1 us vs Hduhu Hduhv x w' as IH1.
-                apply IH1 in Hinvs as [u' [Hinus Hsubu'w']].
-                exists u'. split; try assumption.
-                apply st_trans with (u := w');
+                apply IHHS2 in HR as [a' [b' [HU [HSA HSB]]]].
+                apply IHHS1 in HU as [a'' [b'' [HT [HSA' HSB']]]].
+                exists a''. exists b''. split.
+                + assumption.
+                + split.
+                    * apply st_trans with
+                        (t := a) (u := a') (v := a'');
+                        assumption.
+                    * apply st_trans with
+                        (t := b'') (u := b') (v := b);
+                    assumption.
+            - exists u. exists v. split.
+                + reflexivity.
+                + split; assumption.
+        Qed.
+
+        Lemma inv_rec :
+            forall (t : type) (ts : fields type),
+            subtype t (TRec ts) ->
+            exists (us : fields type),
+            t = TRec us /\ subtype (TRec us) (TRec ts).
+        Proof.
+            intros t ts HS. dependent induction HS.
+            - exists ts. split; auto.
+                apply st_refl.
+            - specialize IHHS2 with (ts0 := ts).
+                assert (HRts : TRec ts = TRec ts);
+                try reflexivity.
+                apply IHHS2 in HRts as IH2.
+                destruct IH2 as [us [HU HSusts]].
+                specialize IHHS1 with (ts := us).
+                apply IHHS1 in HU as IH1.
+                destruct IH1 as [vs [HT HSvsus]].
+                exists vs. split; auto.
+                apply st_trans with 
+                    (t := (TRec vs)) (u := TRec us) (v := TRec ts);
                 assumption.
-        - exists w. split.
-            + apply in_or_app.
-                left. auto.
-            + constructor.
-        - induction H0; inv Hinws.
-            + inv H. inv H5. destruct x0 as [x0 u0].
-                exists u0. split.
-                * constructor. simpl in H2.
-                    rewrite <- H2. reflexivity.
-                * assumption.
-            + inv H. pose proof IHForall2 H8 H2 as HEX.
-                destruct HEX as [u [Hinl HSuw]].
-                exists u. split; try assumption.
-                apply in_cons. assumption.
-        - exists w. apply Permutation_sym in H. split.
-            + apply Permutation_in with (l := ws);
+            - exists (ts ++ vs). split; constructor.
+            - exists us. split; constructor. assumption.
+            - exists us. split; auto.
+                apply st_rec_perm. assumption.
+        Qed.
+    End InvSubsumption.
+
+    Section CanonicalForms.
+        Definition canon_unit (v : expr) : Prop :=
+            value v -> checks v TUnit -> v = EUnit.
+
+        Definition canon_fun (v : expr) : Prop :=
+            forall (a b : type),
+            value v -> checks v (TFun a b) -> 
+            exists (x : id) (t : type) (e : expr), 
+            subtype a t /\ v = EFun x t e.
+
+        Definition canon_rec (v : expr) := 
+            forall (ts : fields type),
+            value v -> checks v (TRec ts) ->
+            exists (es : fields expr) (us : fields type), 
+            v = ERec es /\
+            relfs (check empty) es us /\ 
+            subtype (TRec us) (TRec ts).
+
+        Lemma canonical_forms_unit : 
+            forall (v : expr), canon_unit v.
+        Proof.
+            unfold canon_unit. intros v HV HChk;
+            dependent induction HChk.
+            - apply inv_unit in H as HU. auto.
+            - reflexivity.
+            - inversion HV.
+            - inversion HV.
+            - inversion HV.
+        Qed.
+
+        Lemma canonical_forms_fun :
+            forall (v : expr), canon_fun v.
+        Proof.
+            unfold canon_fun. intros v t t' HV HChk.
+            dependent induction HChk.
+            - apply inv_fun in H as HU.
+                destruct HU as [a' [b' [HF [HSA HSB]]]].
+                specialize IHHChk with
+                    (t := a') (t' := b').
+                pose proof (IHHChk HV HF) as IH.
+                destruct IH as [x [w [e' [HSW HFW]]]].
+                exists x. exists w. exists e'. split.
+                + apply st_trans with
+                    (t := t) (u := a') (v := w);
+                    assumption.
+                + assumption.
+            - inversion HV.
+            - exists x. exists t. exists e. 
+                split; constructor.
+            - inversion HV.
+            - inversion HV.
+        Qed.
+
+        Lemma canonical_forms_rec :
+            forall (v : expr), canon_rec v.
+        Proof.
+            unfold canon_rec. intros v ts HV HChk.
+            dependent induction HChk.
+            - apply inv_rec in H as [us [HU HSusts]].
+                specialize IHHChk with (ts := us).
+                apply IHHChk in HV as IH; auto.
+                destruct IH as [es [vs [Hrec [HR HSvsus]]]].
+                exists es. exists vs. split; auto. split; auto.
+                apply st_trans with
+                    (t := (TRec vs)) (u := (TRec us)) (v := (TRec ts));
                 assumption.
-            + constructor.
-    Qed.
+            - inv HV.
+            - inv HV.
+            - exists es. exists ts. 
+                split; try reflexivity.
+                induction HV; subst; constructor;
+                try assumption;
+                try apply st_refl.
+            - inv HV. 
+        Qed.
+    End CanonicalForms.
 
-    Lemma rec_fields_name :
-        forall (es : fields expr) (ts : fields type),
-        relfs checks es ts ->
-        forall (x : id) (t : type),
-        In (x,t) ts ->
-        exists (e : expr), In (x,e) es.
-    Proof.
-        intros es ts HR. induction HR;
-        intros z t Hints.
-        - inv Hints.
-        - destruct x as (x,e). inv Hints.
-            + exists e. constructor.
-                unfold relf in H.
-                destruct H as [HF _].
-                simpl in *. subst.
-                reflexivity.
-            + apply IHHR in H0 as [e' Hinl].
-                exists e'. apply in_cons.
-                assumption.
-    Qed.
+    Section Progress.
+        Lemma st_fields_name :
+            forall (us ws : fields type),
+            subtype (TRec us) (TRec ws) ->
+            forall (x : id) (w : type),
+            In (x,w) ws ->
+            exists (u : type),
+            In (x,u) us /\ subtype u w.
+        Proof.
+            intros us ws HS.
+            dependent induction HS using IHSubtype; intros x w Hinws.
+            - subst. exists w. 
+                split; auto. constructor.
+            - assert (HSusws : subtype (TRec us) (TRec ws)).
+                + apply st_trans with (u := u); assumption.
+                + pose proof inv_rec u ws HS2 as [vs [Huvs HSvws]]. subst.
+                    assert (Hduhu : TRec us = TRec us);
+                    assert (Hduhv : TRec vs = TRec vs);
+                    assert (Hduhw : TRec ws = TRec ws);
+                    try reflexivity.
+                    pose proof IHHS2 vs ws Hduhv Hduhw x w as IH2.
+                    apply IH2 in Hinws as [w' [Hinvs HSw'w]].
+                    pose proof IHHS1 us vs Hduhu Hduhv x w' as IH1.
+                    apply IH1 in Hinvs as [u' [Hinus Hsubu'w']].
+                    exists u'. split; try assumption.
+                    apply st_trans with (u := w');
+                    assumption.
+            - exists w. split.
+                + apply in_or_app.
+                    left. auto.
+                + constructor.
+            - induction H0; inv Hinws.
+                + inv H. inv H5. destruct x0 as [x0 u0].
+                    exists u0. split.
+                    * constructor. simpl in H2.
+                        rewrite <- H2. reflexivity.
+                    * assumption.
+                + inv H. pose proof IHForall2 H8 H2 as HEX.
+                    destruct HEX as [u [Hinl HSuw]].
+                    exists u. split; try assumption.
+                    apply in_cons. assumption.
+            - exists w. apply Permutation_sym in H. split.
+                + apply Permutation_in with (l := ws);
+                    assumption.
+                + constructor.
+        Qed.
 
-    Definition progress_thm (e : expr) (t : type) : Prop :=
-        checks e t -> value e \/ exists (e' : expr), step e e'.
+        Lemma rec_fields_name :
+            forall (es : fields expr) (ts : fields type),
+            relfs checks es ts ->
+            forall (x : id) (t : type),
+            In (x,t) ts ->
+            exists (e : expr), In (x,e) es.
+        Proof.
+            intros es ts HR. induction HR;
+            intros z t Hints.
+            - inv Hints.
+            - destruct x as (x,e). inv Hints.
+                + exists e. constructor.
+                    unfold relf in H.
+                    destruct H as [HF _].
+                    simpl in *. subst.
+                    reflexivity.
+                + apply IHHR in H0 as [e' Hinl].
+                    exists e'. apply in_cons.
+                    assumption.
+        Qed.
 
-    Lemma var_empty_checks :
-        forall (x : id) (t : type),
-        ~ checks (EVar x) t.
-    Proof.
-        intros x t H. unfold checks in *.
-        remember empty as o in H. 
-        remember (EVar x) as z in H.
-        dependent induction H; 
-        auto; try inv Heqz.
-        discriminate.
-    Qed.
+        Definition progress_thm (e : expr) (t : type) : Prop :=
+            checks e t -> value e \/ exists (e' : expr), step e e'.
 
-    Lemma val_rec_exists :
-        forall (es : fields expr),
-        ~ value (ERec es) <-> Exists (predf (fun e => ~ value e)) es.
-    Proof.
-        intros es. split; intros H.
-        - induction es.
-            + exfalso. apply H.
+        Lemma var_empty_checks :
+            forall (x : id) (t : type),
+            ~ checks (EVar x) t.
+        Proof.
+            intros x t H. unfold checks in *.
+            remember empty as o in H. 
+            remember (EVar x) as z in H.
+            dependent induction H; 
+            auto; try inv Heqz.
+            discriminate.
+        Qed.
+
+        Lemma val_rec_exists :
+            forall (es : fields expr),
+            ~ value (ERec es) <-> Exists (predf (fun e => ~ value e)) es.
+        Proof.
+            intros es. split; intros H.
+            - induction es.
+                + exfalso. apply H.
+                    constructor. constructor.
+                + apply Exists_cons. 
+                    destruct (value_dec (snd a)).
+                    * right. apply IHes. intros V.
+                        inv V. apply H. constructor.
+                        constructor; assumption.
+                    * left. unfold predf. assumption.
+            - intros V. apply Exists_Forall_neg in H.
+                + apply H. inv V. assumption.
+                + pose proof 
+                    (fun x : field expr => 
+                        value_dec (snd x)) as PFV.
+                    intros e. specialize PFV with e.
+                    destruct PFV as [VE | VE]; auto.
+        Qed.
+
+        Lemma val_rec_prefix :
+            forall (es : fields expr),
+            ~ value (ERec es) ->
+            exists (x : id) (e : expr) 
+                (qs rs : fields expr),
+            ~ value e /\ 
+            predfs value qs /\
+            es = qs ++ (x,e) :: rs.
+        Proof.
+            induction es; intros HV.
+            - exfalso. apply HV.
                 constructor. constructor.
-            + apply Exists_cons. 
-                destruct (value_dec (snd a)).
-                * right. apply IHes. intros V.
-                    inv V. apply H. constructor.
-                    constructor; assumption.
-                * left. unfold predf. assumption.
-        - intros V. apply Exists_Forall_neg in H.
-            + apply H. inv V. assumption.
-            + pose proof 
-                (fun x : field expr => 
-                    value_dec (snd x)) as PFV.
-                intros e. specialize PFV with e.
-                destruct PFV as [VE | VE]; auto.
-    Qed.
+            - destruct (value_dec (snd a)).
+                { assert (HVes : ~ value (ERec es)).
+                    - intros HR. apply HV. inv HR.
+                        constructor.
+                        constructor; assumption.
+                    - pose proof IHes HVes as IH.
+                        destruct IH as [x [e [qs [rs [HNV [HPV Hqer]]]]]].
+                        exists x. exists e. exists (a :: qs). 
+                        exists rs. split; try assumption. split.
+                        + constructor; assumption.
+                        + rewrite <- app_comm_cons.
+                            rewrite Hqer. reflexivity. }
+                { exists (fst a). exists (snd a).
+                    exists []. exists es. split;
+                    try assumption. split.
+                    - constructor.
+                    - rewrite app_nil_l. destruct a as (x,e).
+                        reflexivity. }
+        Qed.
 
-    Lemma val_rec_prefix :
-        forall (es : fields expr),
-        ~ value (ERec es) ->
-        exists (x : id) (e : expr) 
-            (qs rs : fields expr),
-        ~ value e /\ 
-        predfs value qs /\
-        es = qs ++ (x,e) :: rs.
-    Proof.
-        induction es; intros HV.
-        - exfalso. apply HV.
-            constructor. constructor.
-        - destruct (value_dec (snd a)).
-            { assert (HVes : ~ value (ERec es)).
-                - intros HR. apply HV. inv HR.
-                    constructor.
-                    constructor; assumption.
-                - pose proof IHes HVes as IH.
-                    destruct IH as [x [e [qs [rs [HNV [HPV Hqer]]]]]].
-                    exists x. exists e. exists (a :: qs). 
-                    exists rs. split; try assumption. split.
-                    + constructor; assumption.
-                    + rewrite <- app_comm_cons.
-                        rewrite Hqer. reflexivity. }
-            { exists (fst a). exists (snd a).
-                exists []. exists es. split;
-                try assumption. split.
-                - constructor.
-                - rewrite app_nil_l. destruct a as (x,e).
-                    reflexivity. }
-    Qed.
+        Theorem Progress :
+            forall (e : expr) (t : type), progress_thm e t.
+        Proof.
+            unfold progress_thm. intros e t HC.
+            unfold checks in *. remember empty as o in HC.
+            dependent induction HC using IHCheck; subst;
+            assert (HE : @empty type = @empty type);
+            try reflexivity.
+            - destruct IHHC as [V | [e' HS]].
+                + reflexivity.
+                + left. assumption.
+                + right. exists e'. assumption.
+            - left. constructor.
+            - discriminate.
+            - left. constructor.
+            - right. pose proof IHHC1 HE as [V | [e1' HS]].
+                + pose proof canonical_forms_fun e1 u v V HC1
+                    as [x [t [e [HS HF]]]].
+                    pose proof sub_exists x e2 e as [e' HSub].
+                    exists e'. subst. constructor. assumption.
+                + exists (EApp e1' e2). constructor. assumption.
+            - induction H2.
+                + left. constructor. constructor.
+                + inv H. inv H1. inv H0. clear H. clear H0. inv H2.
+                    pose proof IHForall2 H7 as IH2.
+                    destruct H2 as [HFXY YES].
+                    pose proof YES HE as [HVX | [e' HSX]].
+                    { destruct (value_dec (ERec l)) as [V | V].
+                        - left. constructor. inv V.
+                            constructor; auto.
+                        - destruct IH2 as [IH2 | IH2]; try contradiction; auto. 
+                            pose proof val_rec_prefix l V as HEX.
+                            destruct HEX as [z [e [qs [rs [HVE [HPV HL]]]]]].
+                            right. subst. destruct IH2 as [e' HS]. inv HS.
+                            exists (ERec (x :: vs ++ (x0,e'0) :: es)).
+                            rewrite app_comm_cons. rewrite app_comm_cons.
+                            constructor; auto.
+                            constructor; auto. }
+                    { right. destruct x as [x e]. simpl in *.
+                        exists (ERec ((x, e') :: l)).
+                        assert (HPV : predfs value []);
+                        try (constructor; constructor).
+                        pose proof step_rec [] l x e e' HPV HSX as HR.
+                        rewrite app_nil_l in HR. rewrite app_nil_l in HR.
+                        assumption. }
+            - right. pose proof IHHC HE as [V | [e' HS]].
+                + pose proof canonical_forms_rec e ts V HC as HCF.
+                    destruct HCF as [es [us [HRec [HR Hsub]]]]; subst.
+                    pose proof st_fields_name us ts Hsub x t H as [u [Hinus HSut]].
+                    pose proof rec_fields_name es us HR x u Hinus as [e' Hines].
+                    exists e'. constructor. assumption.
+                + exists (EPrj e' x). constructor. assumption.
+        Qed.
+    End Progress.
 
-    Theorem Progress :
-        forall (e : expr) (t : type), progress_thm e t.
-    Proof.
-        unfold progress_thm. intros e t HC.
-        unfold checks in *. remember empty as o in HC.
-        dependent induction HC using IHCheck; subst;
-        assert (HE : @empty type = @empty type);
-        try reflexivity.
-        - destruct IHHC as [V | [e' HS]].
-            + reflexivity.
-            + left. assumption.
-            + right. exists e'. assumption.
-        - left. constructor.
-        - discriminate.
-        - left. constructor.
-        - right. pose proof IHHC1 HE as [V | [e1' HS]].
-            + pose proof canonical_forms_fun e1 u v V HC1
-                as [x [t [e [HS HF]]]].
-                pose proof sub_exists x e2 e as [e' HSub].
-                exists e'. subst. constructor. assumption.
-            + exists (EApp e1' e2). constructor. assumption.
-        - induction H2.
-            + left. constructor. constructor.
-            + inv H. inv H1. inv H0. clear H. clear H0. inv H2.
-                pose proof IHForall2 H7 as IH2.
-                destruct H2 as [HFXY YES].
-                pose proof YES HE as [HVX | [e' HSX]].
-                { destruct (value_dec (ERec l)) as [V | V].
-                    - left. constructor. inv V.
-                        constructor; auto.
-                    - destruct IH2 as [IH2 | IH2]; try contradiction; auto. 
-                        pose proof val_rec_prefix l V as HEX.
-                        destruct HEX as [z [e [qs [rs [HVE [HPV HL]]]]]].
-                        right. subst. destruct IH2 as [e' HS]. inv HS.
-                        exists (ERec (x :: vs ++ (x0,e'0) :: es)).
-                        rewrite app_comm_cons. rewrite app_comm_cons.
+    (* Inversion on the Typing Relation. *)
+    Section InvCheck.
+        Lemma inv_chk_fun :
+            forall (g : gamma) (t u v : type) (x : id) (e : expr),
+            check g (EFun x t e) (TFun u v) ->
+            subtype u t /\ check (bind x t g) e v.
+        Proof.
+            intros g t u v x e HC. 
+            dependent induction HC using IHCheck.
+            - pose proof inv_fun u0 u v H as [a [b [Huab [Hua Hbv]]]].
+                subst. assert (HEFun : EFun x t e = EFun x t e);
+                assert (HTFun : TFun a b = TFun a b); try reflexivity.
+                pose proof IHHC t a b x e HEFun HTFun as IH.
+                destruct IH as [HS HCB]. split.
+                + apply st_trans with (u := a); assumption.
+                + apply check_subsume with (u := b); assumption.
+            - split; try apply st_refl. assumption.
+        Qed.
+
+        Lemma inv_chk_rec :
+            forall (g : gamma) (es : fields expr) (ts : fields type),
+            check g (ERec es) (TRec ts) ->
+            forall (x : id) (t : type),
+            In (x,t) ts ->
+            exists (e : expr), 
+            In (x,e) es /\ check g e t.
+        Proof.
+            intros g es ts HC x t Hints.
+            dependent induction HC using IHCheck.
+            - pose proof inv_rec u ts H as HRu.
+                destruct HRu as [us [Huus HSus]].
+                assert (HERec : ERec es = ERec es);
+                try reflexivity.
+                pose proof st_fields_name us ts HSus x t Hints as HT.
+                destruct HT as [w [Hinus HSut]].
+                pose proof IHHC es us HERec Huus x w Hinus as IH.
+                destruct IH as [e [Hines HCew]]. exists e. split.
+                + assumption.
+                + apply check_subsume with (u := w);
+                    assumption.
+            - induction H2; inv Hints;
+                inv H; inv H0; clear H; clear H0;
+                inv H1; clear H1.
+                + destruct x0 as [x0 e0]. exists e0. 
+                    destruct H5 as [Hfst Hck].
+                    simpl in *; subst. split.
+                    * left. reflexivity.
+                    * assumption.
+                + pose proof IHForall2 H8 H10 H12 H4 as IH. 
+                    destruct IH as [e [HIN HCK]].
+                    exists e. split; try assumption.
+                    apply in_cons. assumption.
+        Qed.
+
+        Lemma inv_chk_rec' :
+            forall (g : gamma) (es : fields expr) (ts : fields type),
+            check g (ERec es) (TRec ts) ->
+            forall (x : id) (t : type),
+            In (x,t) ts ->
+            forall (e : expr),
+            In (x,e) es ->
+            check g e t.
+        Proof.
+            intros g es ts HC x t Hints.
+            intros f Hinfes.
+            dependent induction HC using IHCheck.
+            - apply inv_rec in H as [us [Huus HSusts]].
+                pose proof st_fields_name 
+                    us ts HSusts x t Hints as SFN.
+                destruct SFN as [w [Hinus HSwt]].
+                apply check_subsume with (u := w); auto.
+                apply IHHC with (es0 := es) (ts := us) (x := x);
+                auto. 
+            - assert (HC : check g (ERec es) (TRec ts)).
+                + constructor; auto.
+                + pose proof inv_chk_rec g es ts 
+                    HC x t Hints as ICR.
+                    destruct ICR as [e [Hin Hget]].
+                    pose proof relfs_nodup_eq es x e f 
+                        H Hin Hinfes as EF. subst.
+                        assumption.                  
+        Qed.
+    End InvCheck.
+
+    Section SubstitutionLemma.
+        Lemma bind_unfree_var :
+            forall (e : expr) (x : id) (u v : type) (g : gamma),
+            ~ IS.In x (fv e) ->
+            check g e u <-> check (bind x v g) e u.
+        Proof.
+            intros e x u v g HN. split; intros HC;
+            dependent induction HC using IHCheck.
+            - pose proof IHHC HN as IH.
+                apply check_subsume with (u := u);
+                assumption.
+            - constructor.
+            - constructor. simpl in *.
+                assert (Hxx0 : x <> x0).
+                + intros Hxx0. apply HN. subst.
+                    constructor. reflexivity.
+                + apply bind_complete; assumption.
+            - constructor. destruct (IdDec.eq_dec x x0) as [HX | HX]; subst.
+                + rewrite <- rebind_correct. assumption.
+                + simpl in *. assert (HNin : ~ IS.In x (fv e)).
+                    * intros HNin. apply HN.
+                        apply not_eq_sym in HX.
+                        apply ISF.remove_2; assumption.
+                    * pose proof bind_diff_comm x x0 v u g HX as BDC.
+                        rewrite <- BDC. pose proof IHHC HNin as IH.
+                        assumption.
+            - simpl in *. apply check_app with (u := u).
+                + apply IHHC1. intros H1. apply HN.
+                    apply ISF.union_2. assumption.
+                + apply IHHC2. intros H2. apply HN.
+                    apply ISF.union_3. assumption.
+            - constructor; auto. clear H. clear H0.
+                induction H2;
+                constructor; inv H1; inv H.
+                + split; try assumption. apply H3.
+                    intros Hxx0. apply HN. simpl.
+                    apply ISF.union_3. assumption.
+                + assert (Hxl : ~ IS.In x (fv (ERec l))).
+                    * intros Hxl. apply HN. simpl in *.
+                        apply ISF.union_2. assumption.
+                    * apply (IHForall2 Hxl H7).
+            - simpl in *. apply check_prj with (ts := ts);
+                try assumption. auto.
+            - pose proof IHHC x v g HN as IH.
+                apply check_subsume with (u := u); auto.
+            - constructor.
+            - simpl in *. constructor.
+                assert (Hxx0 : x <> x0).
+                + intros Hxx0. apply HN. subst.
+                    constructor. reflexivity.
+                + apply bind_complete in H; assumption.
+            - constructor. destruct (IdDec.eq_dec x x0) as [HX | HX]; subst.
+                + rewrite <- rebind_correct in HC. assumption.
+                + simpl in *. assert (HNin : ~ IS.In x (fv e)).
+                    * intros HNin. apply HN.
+                        apply not_eq_sym in HX.
+                        apply ISF.remove_2; assumption.
+                    * pose proof bind_diff_comm x x0 v u g HX as BDC.
+                        symmetry in BDC.
+                        pose proof IHHC x v (bind x0 u g) HNin BDC as IH.
+                        apply IH.
+            - simpl in *. apply check_app with (u := u).
+                + apply IHHC1 with (x0 := x) (v1 := v); 
+                    auto. intros H1. apply HN. 
+                    apply ISF.union_2. assumption.
+                + apply IHHC2 with (x0 := x) (v0 := v); 
+                    auto. intros H2. apply HN. 
+                    apply ISF.union_3. assumption.
+            - constructor; auto. induction H2; 
+                constructor; inv H; inv H0;
+                clear H; clear H0; inv H1; inv H2; inv H5.
+                + split; try assumption.
+                    apply H0 with (x1 := x) (v0 := v); auto.
+                    intros Hxx0. apply HN. simpl.
+                    apply ISF.union_3. assumption.
+                + assert (Hxl : ~ IS.In x (fv (ERec l))).
+                    * intros Hxl. apply HN. simpl in *.
+                        apply ISF.union_2. assumption.
+                    * apply (IHForall2 H7 H9 H11 Hxl).
+            - apply check_prj with (ts := ts); auto.
+                simpl in *. assert (HR : bind x v g = bind x v g);
+                try reflexivity. pose proof IHHC x v g HN HR as IH.
+                assumption.
+        Qed.
+
+        Definition substitution_lemma (x : id) (esub e e' : expr) :=
+            sub x esub e e' ->
+            forall (u v : type) (g : gamma),
+            check (bind x u g) e v -> 
+            check g esub u -> 
+            check g e' v.
+
+        Lemma fields_sub_nodups :
+            forall (x : id) (esub : expr) (es es' : fields expr),
+            relfs (sub x esub) es es' ->
+            nodupfs es -> nodupfs es'.
+        Proof.
+            intros x esub es es' HS.
+            induction HS; intros ND.
+            - constructor.
+            - destruct x0 as [x0 ex0].
+                destruct y as [y ey].
+                destruct H as [Hfst Hsub].
+                simpl in *. subst.
+                inv ND.
+                unfold nodupfs in *. simpl in *.
+                constructor; simpl in *; auto.
+                intros Hin. apply H1.
+                pose proof relfs_name_share (sub x esub) as RNS.
+                apply RNS with (x0 := y) in HS. 
+                apply HS. assumption.
+        Qed.
+
+        Lemma SubstitutionLem :
+            forall (x : id) (esub e e' : expr),
+            substitution_lemma x esub e e'.
+        Proof.
+            intros x esub e e' HS.
+            induction HS using IHSubstitute;
+            intros u v g HCB;
+            remember g as g' in HCB; 
+            dependent induction HCB; intros HC;
+            try (apply check_subsume with (u := u0); auto;
+                apply IHHCB with (x0 := x) (u1 := u) (g' := g); 
+                try reflexivity; assumption);
+            assert (Hgg : g = g); try reflexivity.
+            - constructor.
+            - rewrite bind_correct in H. injintrosubst H. auto.
+            - apply bind_complete in H0 as BC; auto.
+                constructor. auto.
+            - constructor. clear IHHCB. 
+                rewrite <- rebind_correct in HCB.
+                assumption.
+            - pose proof IHHCB g Hgg u e t y 
+                H0 x H HS IHHS as IH.
+                apply check_subsume with (u := u0); auto.
+            - clear IHHCB. constructor.
+                rewrite <- (bind_diff_comm x y u t g H) in HCB.
+                apply IHHS in HCB as IH; auto.
+                apply bind_unfree_var; auto.
+            - pose proof IHHCB g Hgg u H3 e H4 t y 
+                H1 H2 HS1 IHHS1 x H H0 HS2 IHHS2 as IH.
+                apply check_subsume with (u := u0); auto.
+            - clear IHHCB. constructor.
+                apply IHHS2 with (u := u).
+                { apply IHHS1 with (u := t).
+                    - pose proof bind_diff_comm 
+                        x z u t g H0 as BDC1.
+                        rewrite BDC1.
+                        pose proof bind_diff_comm
+                            y z t t (bind x u g) H1 as BDC2.
+                        rewrite BDC2. apply bind_unfree_var; auto.
+                    - apply bind_unfree_var.
+                        + intros Hin. simpl in *.
+                            apply IS.singleton_spec in Hin.
+                            contradiction.
+                        + constructor. apply bind_correct. }
+                { apply bind_unfree_var; auto. }
+            - pose proof IHHCB x e1 e2 HS1 HS2
+                IHHS1 IHHS2 u g as IH.
+                apply check_subsume with (u := u0); auto.
+            - clear IHHCB1. clear IHHCB2.
+                apply check_app with (u := u0).
+                + apply IHHS1 with (u := u); auto.
+                + apply IHHS2 with (u := u); auto.
+            - pose proof IHHCB x fs H H0 u g as IH.
+                apply check_subsume with (u := u0); auto. 
+            - apply check_rec; auto.
+                + apply fields_sub_nodups in H; auto.
+                + generalize dependent fs'.
+                induction H1; intros fs';
+                intros HSfs; intros Hbig;
+                inv HSfs; constructor; auto;
+                destruct x0 as [x0 ex0];
+                destruct y as [y ey];
+                destruct y0 as [y0 ey0];
+                destruct H5 as [Hfst Hsub];
+                inv HSfs; clear HSfs;
+                inv Hbig; clear Hbig;
+                destruct H8 as [Hfst' Hck];
+                destruct H as [Hyy0 Hcky];
+                simpl in *; subst; clear Hfst'.
+                * split; auto; simpl. 
+                    apply Hck with (u := u); auto.
+                * inv H2; clear H2.
+                    inv H3; clear H3. clear H4. clear H2.
+                    pose proof IHForall2 H5 H8
+                        l'0 H9 H11 as IH; clear IHForall2.
+                    apply IH.
+            - pose proof IHHCB x e y HS  IHHS u g as IH.
+                apply check_subsume with (u := u0); auto.
+            - clear IHHCB. apply check_prj with (ts := ts); auto.
+                apply IHHS in HCB as IH; auto.
+        Qed.
+    End SubstitutionLemma.
+
+    Section Preservation.
+        Definition preservation (e e' : expr) : Prop :=
+            step e e' -> forall (t : type),
+            checks e t -> checks e' t.
+
+        Theorem Preservation :
+            forall (e e' : expr), preservation e e'.
+        Proof.
+            intros e e' HS.
+            dependent induction HS; intros u HC;
+            unfold checks in *;
+            remember empty as o in HC.
+            - dependent induction HC.
+                + apply check_subsume with (u := u); auto.
+                    apply IHHC with (x0 := x) (t0 := t)
+                    (e0 := e) (es0 := es); auto.
+                + clear IHHC1. clear IHHC2.
+                    apply inv_chk_fun in HC1 as [HSut Hev].
+                    apply SubstitutionLem in H as SL.
+                    apply SL with (u := t); auto.
+                    apply check_subsume with (u := u); auto.
+            - dependent induction HC.
+                + apply check_subsume with (u := u); auto.
+                    apply IHHC with (e3 := e1) (e4 := e2); auto.
+                + clear IHHC1. clear IHHC2.
+                    apply check_app with (u := u); auto.
+            - generalize dependent e.
+                dependent induction HC;
+                intros e Hin.
+                + apply check_subsume with (u := u); auto.
+                    apply IHHC with (es0 := es) (x0 := x); auto.
+                + clear IHHC.
+                    pose proof inv_chk_rec' empty 
+                        es ts HC x t H e Hin as ICR.
+                    assumption.
+            - dependent induction HC.
+                + apply check_subsume with (u := u); auto.
+                    apply IHHC with (e0 := e) (x0 := x); auto.
+                + clear IHHC. apply check_prj with (ts := ts); auto.
+            - dependent induction HC.
+                { apply check_subsume with (u := u); auto.
+                    apply IHHC with (e0 := e) 
+                        (x0 := x) (es0 := es) (vs0 := vs); auto. }
+                { constructor; auto.
+                    - unfold nodupfs in *.
+                        rewrite map_app.
+                        rewrite map_app in H2.
+                        simpl in *. assumption.
+                    - apply relfs_app in H1 as RA.
+                        destruct RA as [ts1 [ts2 [Hts [Hts1 Hts2]]]].
+                        subst. inv Hts2.
+                        inv H5. apply IHHS in H4.
+                        apply relfs_app_dist; auto.
                         constructor; auto.
                         constructor; auto. }
-                { right. destruct x as [x e]. simpl in *.
-                    exists (ERec ((x, e') :: l)).
-                    assert (HPV : predfs value []);
-                    try (constructor; constructor).
-                    pose proof step_rec [] l x e e' HPV HSX as HR.
-                    rewrite app_nil_l in HR. rewrite app_nil_l in HR.
-                    assumption. }
-        - right. pose proof IHHC HE as [V | [e' HS]].
-            + pose proof canonical_forms_rec e ts V HC as HCF.
-                destruct HCF as [es [us [HRec [HR Hsub]]]]; subst.
-                pose proof st_fields_name us ts Hsub x t H as [u [Hinus HSut]].
-                pose proof rec_fields_name es us HR x u Hinus as [e' Hines].
-                exists e'. constructor. assumption.
-            + exists (EPrj e' x). constructor. assumption.
-    Qed.
-End Progress.
-
-(* Inversion on the Typing Relation. *)
-Section InvCheck.
-    Lemma inv_chk_fun :
-        forall (g : gamma) (t u v : type) (x : id) (e : expr),
-        check g (EFun x t e) (TFun u v) ->
-        subtype u t /\ check (bind x t g) e v.
-    Proof.
-        intros g t u v x e HC. 
-        dependent induction HC using IHCheck.
-        - pose proof inv_fun u0 u v H as [a [b [Huab [Hua Hbv]]]].
-            subst. assert (HEFun : EFun x t e = EFun x t e);
-            assert (HTFun : TFun a b = TFun a b); try reflexivity.
-            pose proof IHHC t a b x e HEFun HTFun as IH.
-            destruct IH as [HS HCB]. split.
-            + apply st_trans with (u := a); assumption.
-            + apply check_subsume with (u := b); assumption.
-        - split; try apply st_refl. assumption.
-    Qed.
-
-    Lemma inv_chk_rec :
-        forall (g : gamma) (es : fields expr) (ts : fields type),
-        check g (ERec es) (TRec ts) ->
-        forall (x : id) (t : type),
-        In (x,t) ts ->
-        exists (e : expr), 
-        In (x,e) es /\ check g e t.
-    Proof.
-        intros g es ts HC x t Hints.
-        dependent induction HC using IHCheck.
-        - pose proof inv_rec u ts H as HRu.
-            destruct HRu as [us [Huus HSus]].
-            assert (HERec : ERec es = ERec es);
-            try reflexivity.
-            pose proof st_fields_name us ts HSus x t Hints as HT.
-            destruct HT as [w [Hinus HSut]].
-            pose proof IHHC es us HERec Huus x w Hinus as IH.
-            destruct IH as [e [Hines HCew]]. exists e. split.
-            + assumption.
-            + apply check_subsume with (u := w);
-                assumption.
-        - induction H2; inv Hints;
-            inv H; inv H0; clear H; clear H0;
-            inv H1; clear H1.
-            + destruct x0 as [x0 e0]. exists e0. 
-                destruct H5 as [Hfst Hck].
-                simpl in *; subst. split.
-                * left. reflexivity.
-                * assumption.
-            + pose proof IHForall2 H8 H10 H12 H4 as IH. 
-                destruct IH as [e [HIN HCK]].
-                exists e. split; try assumption.
-                apply in_cons. assumption.
-    Qed.
-
-    Lemma inv_chk_rec' :
-        forall (g : gamma) (es : fields expr) (ts : fields type),
-        check g (ERec es) (TRec ts) ->
-        forall (x : id) (t : type),
-        In (x,t) ts ->
-        forall (e : expr),
-        In (x,e) es ->
-        check g e t.
-    Proof.
-        intros g es ts HC x t Hints.
-        intros f Hinfes.
-        dependent induction HC using IHCheck.
-        - apply inv_rec in H as [us [Huus HSusts]].
-            pose proof st_fields_name 
-                us ts HSusts x t Hints as SFN.
-            destruct SFN as [w [Hinus HSwt]].
-            apply check_subsume with (u := w); auto.
-            apply IHHC with (es0 := es) (ts := us) (x := x);
-            auto. 
-        - assert (HC : check g (ERec es) (TRec ts)).
-            + constructor; auto.
-            + pose proof inv_chk_rec g es ts 
-                HC x t Hints as ICR.
-                destruct ICR as [e [Hin Hget]].
-                pose proof relfs_nodup_eq es x e f 
-                    H Hin Hinfes as EF. subst.
-                    assumption.                  
-    Qed.
-End InvCheck.
-
-Section SubstitutionLemma.
-    Lemma bind_unfree_var :
-        forall (e : expr) (x : id) (u v : type) (g : gamma),
-        ~ IS.In x (fv e) ->
-        check g e u <-> check (bind x v g) e u.
-    Proof.
-        intros e x u v g HN. split; intros HC;
-        dependent induction HC using IHCheck.
-        - pose proof IHHC HN as IH.
-            apply check_subsume with (u := u);
-            assumption.
-        - constructor.
-        - constructor. simpl in *.
-            assert (Hxx0 : x <> x0).
-            + intros Hxx0. apply HN. subst.
-                constructor. reflexivity.
-            + apply bind_complete; assumption.
-        - constructor. destruct (IdDec.eq_dec x x0) as [HX | HX]; subst.
-            + rewrite <- rebind_correct. assumption.
-            + simpl in *. assert (HNin : ~ IS.In x (fv e)).
-                * intros HNin. apply HN.
-                    apply not_eq_sym in HX.
-                    apply ISF.remove_2; assumption.
-                * pose proof bind_diff_comm x x0 v u g HX as BDC.
-                    rewrite <- BDC. pose proof IHHC HNin as IH.
-                    assumption.
-        - simpl in *. apply check_app with (u := u).
-            + apply IHHC1. intros H1. apply HN.
-                apply ISF.union_2. assumption.
-            + apply IHHC2. intros H2. apply HN.
-                apply ISF.union_3. assumption.
-        - constructor; auto. clear H. clear H0.
-            induction H2;
-            constructor; inv H1; inv H.
-            + split; try assumption. apply H3.
-                intros Hxx0. apply HN. simpl.
-                apply ISF.union_3. assumption.
-            + assert (Hxl : ~ IS.In x (fv (ERec l))).
-                * intros Hxl. apply HN. simpl in *.
-                    apply ISF.union_2. assumption.
-                * apply (IHForall2 Hxl H7).
-        - simpl in *. apply check_prj with (ts := ts);
-            try assumption. auto.
-        - pose proof IHHC x v g HN as IH.
-            apply check_subsume with (u := u); auto.
-        - constructor.
-        - simpl in *. constructor.
-            assert (Hxx0 : x <> x0).
-            + intros Hxx0. apply HN. subst.
-                constructor. reflexivity.
-            + apply bind_complete in H; assumption.
-        - constructor. destruct (IdDec.eq_dec x x0) as [HX | HX]; subst.
-            + rewrite <- rebind_correct in HC. assumption.
-            + simpl in *. assert (HNin : ~ IS.In x (fv e)).
-                * intros HNin. apply HN.
-                    apply not_eq_sym in HX.
-                    apply ISF.remove_2; assumption.
-                * pose proof bind_diff_comm x x0 v u g HX as BDC.
-                    symmetry in BDC.
-                    pose proof IHHC x v (bind x0 u g) HNin BDC as IH.
-                    apply IH.
-        - simpl in *. apply check_app with (u := u).
-            + apply IHHC1 with (x0 := x) (v1 := v); 
-                auto. intros H1. apply HN. 
-                apply ISF.union_2. assumption.
-            + apply IHHC2 with (x0 := x) (v0 := v); 
-                auto. intros H2. apply HN. 
-                apply ISF.union_3. assumption.
-        - constructor; auto. induction H2; 
-            constructor; inv H; inv H0;
-            clear H; clear H0; inv H1; inv H2; inv H5.
-            + split; try assumption.
-                apply H0 with (x1 := x) (v0 := v); auto.
-                intros Hxx0. apply HN. simpl.
-                apply ISF.union_3. assumption.
-            + assert (Hxl : ~ IS.In x (fv (ERec l))).
-                * intros Hxl. apply HN. simpl in *.
-                    apply ISF.union_2. assumption.
-                * apply (IHForall2 H7 H9 H11 Hxl).
-        - apply check_prj with (ts := ts); auto.
-            simpl in *. assert (HR : bind x v g = bind x v g);
-            try reflexivity. pose proof IHHC x v g HN HR as IH.
-            assumption.
-    Qed.
-
-    Definition substitution_lemma (x : id) (esub e e' : expr) :=
-        sub x esub e e' ->
-        forall (u v : type) (g : gamma),
-        check (bind x u g) e v -> 
-        check g esub u -> 
-        check g e' v.
-
-    Lemma fields_sub_nodups :
-        forall (x : id) (esub : expr) (es es' : fields expr),
-        relfs (sub x esub) es es' ->
-        nodupfs es -> nodupfs es'.
-    Proof.
-        intros x esub es es' HS.
-        induction HS; intros ND.
-        - constructor.
-        - destruct x0 as [x0 ex0].
-            destruct y as [y ey].
-            destruct H as [Hfst Hsub].
-            simpl in *. subst.
-            inv ND.
-            unfold nodupfs in *. simpl in *.
-            constructor; simpl in *; auto.
-            intros Hin. apply H1.
-            pose proof relfs_name_share (sub x esub) as RNS.
-            apply RNS with (x0 := y) in HS. 
-            apply HS. assumption.
-    Qed.
-
-    Lemma SubstitutionLem :
-        forall (x : id) (esub e e' : expr),
-        substitution_lemma x esub e e'.
-    Proof.
-        intros x esub e e' HS.
-        induction HS using IHSubstitute;
-        intros u v g HCB;
-        remember g as g' in HCB; 
-        dependent induction HCB; intros HC;
-        try (apply check_subsume with (u := u0); auto;
-            apply IHHCB with (x0 := x) (u1 := u) (g' := g); 
-            try reflexivity; assumption);
-        assert (Hgg : g = g); try reflexivity.
-        - constructor.
-        - rewrite bind_correct in H. injintrosubst H. auto.
-        - apply bind_complete in H0 as BC; auto.
-            constructor. auto.
-        - constructor. clear IHHCB. 
-            rewrite <- rebind_correct in HCB.
-            assumption.
-        - pose proof IHHCB g Hgg u e t y 
-            H0 x H HS IHHS as IH.
-            apply check_subsume with (u := u0); auto.
-        - clear IHHCB. constructor.
-            rewrite <- (bind_diff_comm x y u t g H) in HCB.
-            apply IHHS in HCB as IH; auto.
-            apply bind_unfree_var; auto.
-        - pose proof IHHCB g Hgg u H3 e H4 t y 
-            H1 H2 HS1 IHHS1 x H H0 HS2 IHHS2 as IH.
-            apply check_subsume with (u := u0); auto.
-        - clear IHHCB. constructor.
-            apply IHHS2 with (u := u).
-            { apply IHHS1 with (u := t).
-                - pose proof bind_diff_comm 
-                    x z u t g H0 as BDC1.
-                    rewrite BDC1.
-                    pose proof bind_diff_comm
-                        y z t t (bind x u g) H1 as BDC2.
-                    rewrite BDC2. apply bind_unfree_var; auto.
-                - apply bind_unfree_var.
-                    + intros Hin. simpl in *.
-                        apply IS.singleton_spec in Hin.
-                        contradiction.
-                    + constructor. apply bind_correct. }
-            { apply bind_unfree_var; auto. }
-        - pose proof IHHCB x e1 e2 HS1 HS2
-            IHHS1 IHHS2 u g as IH.
-            apply check_subsume with (u := u0); auto.
-        - clear IHHCB1. clear IHHCB2.
-            apply check_app with (u := u0).
-            + apply IHHS1 with (u := u); auto.
-            + apply IHHS2 with (u := u); auto.
-        - pose proof IHHCB x fs H H0 u g as IH.
-            apply check_subsume with (u := u0); auto. 
-        - apply check_rec; auto.
-            + apply fields_sub_nodups in H; auto.
-            + generalize dependent fs'.
-            induction H1; intros fs';
-            intros HSfs; intros Hbig;
-            inv HSfs; constructor; auto;
-            destruct x0 as [x0 ex0];
-            destruct y as [y ey];
-            destruct y0 as [y0 ey0];
-            destruct H5 as [Hfst Hsub];
-            inv HSfs; clear HSfs;
-            inv Hbig; clear Hbig;
-            destruct H8 as [Hfst' Hck];
-            destruct H as [Hyy0 Hcky];
-            simpl in *; subst; clear Hfst'.
-            * split; auto; simpl. 
-                apply Hck with (u := u); auto.
-            * inv H2; clear H2.
-                inv H3; clear H3. clear H4. clear H2.
-                pose proof IHForall2 H5 H8
-                    l'0 H9 H11 as IH; clear IHForall2.
-                apply IH.
-        - pose proof IHHCB x e y HS  IHHS u g as IH.
-            apply check_subsume with (u := u0); auto.
-        - clear IHHCB. apply check_prj with (ts := ts); auto.
-            apply IHHS in HCB as IH; auto.
-    Qed.
-End SubstitutionLemma.
-
-Section Preservation.
-    Definition preservation (e e' : expr) : Prop :=
-        step e e' -> forall (t : type),
-        checks e t -> checks e' t.
-
-    Theorem Preservation :
-        forall (e e' : expr), preservation e e'.
-    Proof.
-        intros e e' HS.
-        dependent induction HS; intros u HC;
-        unfold checks in *;
-        remember empty as o in HC.
-        - dependent induction HC.
-            + apply check_subsume with (u := u); auto.
-                apply IHHC with (x0 := x) (t0 := t)
-                (e0 := e) (es0 := es); auto.
-            + clear IHHC1. clear IHHC2.
-                apply inv_chk_fun in HC1 as [HSut Hev].
-                apply SubstitutionLem in H as SL.
-                apply SL with (u := t); auto.
-                apply check_subsume with (u := u); auto.
-        - dependent induction HC.
-            + apply check_subsume with (u := u); auto.
-                apply IHHC with (e3 := e1) (e4 := e2); auto.
-            + clear IHHC1. clear IHHC2.
-                apply check_app with (u := u); auto.
-        - generalize dependent e.
-            dependent induction HC;
-            intros e Hin.
-            + apply check_subsume with (u := u); auto.
-                apply IHHC with (es0 := es) (x0 := x); auto.
-            + clear IHHC.
-                pose proof inv_chk_rec' empty 
-                    es ts HC x t H e Hin as ICR.
-                assumption.
-        - dependent induction HC.
-            + apply check_subsume with (u := u); auto.
-                apply IHHC with (e0 := e) (x0 := x); auto.
-            + clear IHHC. apply check_prj with (ts := ts); auto.
-        - dependent induction HC.
-            { apply check_subsume with (u := u); auto.
-                apply IHHC with (e0 := e) 
-                    (x0 := x) (es0 := es) (vs0 := vs); auto. }
-            { constructor; auto.
-                - unfold nodupfs in *.
-                    rewrite map_app.
-                    rewrite map_app in H2.
-                    simpl in *. assumption.
-                - apply relfs_app in H1 as RA.
-                    destruct RA as [ts1 [ts2 [Hts [Hts1 Hts2]]]].
-                    subst. inv Hts2.
-                    inv H5. apply IHHS in H4.
-                    apply relfs_app_dist; auto.
-                    constructor; auto.
-                    constructor; auto. }
-    Qed.
-End Preservation.
+        Qed.
+    End Preservation.
 End SubsumptionSTLC.
 
 Definition map_pair {A B C D : Type} 
@@ -1464,374 +1503,458 @@ Definition map_snd {A B C : Type} (f : B -> C) : A * B -> A * C :=
     map_pair ID f.
 
 Module Coercion.
-Module SS := SubsumptionSTLC.
+    Module SS := SubsumptionSTLC.
+    Module SST := SS.SSType.
+    Module SSE := SS.SSExpr.
 
-Inductive type : Type :=
-    | TUnit
-    | TFun (t t' : type)
-    | TRec (ts : fields type).
+    Inductive type : Type :=
+        | TUnit
+        | TFun (t t' : type)
+        | TRec (ts : fields type).
 
-Inductive expr : Type :=
-    | EUnit
-    | EVar (x : id)
-    | EFun (x : id) (t : type) (e : expr)
-    | EApp (e1 e2 : expr)
-    | ERec (es : fields expr)
-    | EPrj (e : expr) (x : id).
+    Inductive expr : Type :=
+        | EUnit
+        | EVar (x : id)
+        | EFun (x : id) (t : type) (e : expr)
+        | EApp (e1 e2 : expr)
+        | ERec (es : fields expr)
+        | EPrj (e : expr) (x : id).
 
-(* free variables *)
-Fixpoint fv (e : expr) : IS.t :=
-    match e with
-    | EUnit => IS.empty
-    | EVar x => IS.singleton x
-    | EFun x _ e => IS.remove x (fv e)
-    | EApp e1 e2 => IS.union (fv e1) (fv e2)
-    | ERec (es) => 
-        fold_right 
-            (fun (e : field expr) acc => 
-                IS.union acc (fv (snd e)))
-            IS.empty es
-    | EPrj e _ => fv e
-    end.
+    (* free variables *)
+    Fixpoint fv (e : expr) : IS.t :=
+        match e with
+        | EUnit => IS.empty
+        | EVar x => IS.singleton x
+        | EFun x _ e => IS.remove x (fv e)
+        | EApp e1 e2 => IS.union (fv e1) (fv e2)
+        | ERec (es) => 
+            fold_right 
+                (fun (e : field expr) acc => 
+                    IS.union acc (fv (snd e)))
+                IS.empty es
+        | EPrj e _ => fv e
+        end.
 
-Inductive check (g : @gamma type) : expr -> type -> Prop :=
-    | check_unit : check g EUnit TUnit
-    | check_var : forall (x : id) (t : type),
-        g x = Some t ->
-        check g (EVar x) t
-    | check_fun : forall (x : id) (t t' : type) (e : expr),
-        check (bind x t g) e t' ->
-        check g (EFun x t e) (TFun t t')
-    | check_app : forall (e1 e2 : expr) (t t' : type),
-        check g e1 (TFun t t') ->
-        check g e2 t ->
-        check g (EApp e1 e2) t'
-    | check_rec : forall (es : fields expr) (ts : fields type),
-        relfs (check g) es ts ->
-        check g (ERec es) (TRec ts)
-    | check_prj : forall (e : expr) (x : id) (t : type) (ts : fields type),
-        In (x,t) ts ->
-        check g e (TRec ts) ->
-        check g (EPrj e x) t.
+    Inductive check (g : @gamma type) : expr -> type -> Prop :=
+        | check_unit : check g EUnit TUnit
+        | check_var : forall (x : id) (t : type),
+            g x = Some t ->
+            check g (EVar x) t
+        | check_fun : forall (x : id) (t t' : type) (e : expr),
+            check (bind x t g) e t' ->
+            check g (EFun x t e) (TFun t t')
+        | check_app : forall (e1 e2 : expr) (t t' : type),
+            check g e1 (TFun t t') ->
+            check g e2 t ->
+            check g (EApp e1 e2) t'
+        | check_rec : forall (es : fields expr) (ts : fields type),
+            relfs (check g) es ts ->
+            check g (ERec es) (TRec ts)
+        | check_prj : forall (e : expr) (x : id) (t : type) (ts : fields type),
+            In (x,t) ts ->
+            check g e (TRec ts) ->
+            check g (EPrj e x) t.
 
-Fixpoint translate_type (t : SS.type) : type :=
-    match t with
-    | SS.TTop | SS.TUnit => TUnit
-    | SS.TFun t t' => 
-        TFun (translate_type t) (translate_type t')
-    | SS.TRec ts =>
-        TRec (map (map_snd translate_type) ts)
-    end.
+    Fixpoint translate_type (t : SST.type) : type :=
+        match t with
+        | SST.TTop | SST.TUnit => TUnit
+        | SST.TFun t t' => 
+            TFun (translate_type t) (translate_type t')
+        | SST.TRec ts =>
+            TRec (map (map_snd translate_type) ts)
+        end.
 
-(* Why Coq:
-    Incorrect elimination of "HS'" in the inductive type "Forall2":
-    the return type has sort "Type" while it should be "Prop".
-    Elimination of an inductive object of sort Prop
-    is not allowed on a predicate in sort Type
-    because proofs can be eliminated only to build proofs. *)
-Fail Fixpoint rechelp {ss' ts' : fields SS.type} 
-(HS' : relfs SS.subtype ss' ts') : fields expr :=
-    match HS' with
-    | Forall2_nil _ => []
-    | Forall2_cons s _ (conj _ Hst) Hssts =>
-        (fst s, EUnit) :: (rechelp Hssts)
-    end.
+    (* Why Coq:
+        Incorrect elimination of "HS'" in the inductive type "Forall2":
+        the return type has sort "Type" while it should be "Prop".
+        Elimination of an inductive object of sort Prop
+        is not allowed on a predicate in sort Type
+        because proofs can be eliminated only to build proofs. *)
+    Fail Fixpoint rechelp {ss' ts' : fields SST.type} 
+    (HS' : relfs SS.subtype ss' ts') : fields expr :=
+        match HS' with
+        | Forall2_nil _ => []
+        | Forall2_cons s _ (conj _ Hst) Hssts =>
+            (fst s, EUnit) :: (rechelp Hssts)
+        end.
 
-(* why Coq, why? I cannot define the translation
-    as a function from subtyping derivations 
-    to types... :( *)
-Fail Fixpoint translate_subtype {u v : SS.type} (HS : SS.subtype u v) : expr :=
-    let x := EVar "x" in
-    let f := EVar "f" in
-    let r := EVar "r" in
-    match HS with
-    | SS.st_refl t => EFun "x" (translate_type t) x
-    | SS.st_trans s _ _ HSsu HSut => 
-        EFun "x" (translate_type s) 
-            (EApp (translate_subtype HSsu)
-                (EApp (translate_subtype HSut) x))
-    | SS.st_top t => EFun "x" (translate_type t) EUnit
-    | SS.st_fun s1 s2 t1 _ C1 C2 =>
-        EFun "f" (translate_type (SS.TFun s1 s2 ))
-            (EFun "x" (translate_type t1) 
-                (EApp (translate_subtype C2) 
-                    (EApp f
-                        (EApp (translate_subtype C1) x))))
-    | SS.st_rec_width us vs =>
-        EFun "r" 
-            (TRec (map (map_snd translate_type) (us ++ vs)))
-            (ERec 
-                (map 
-                    (fun (u : field SS.type) => 
-                        (fst u, (EPrj r (fst u)))) 
-                    us))
-    | SS.st_rec_depth ss _ HS =>
-        let fix rechelp {ss' ts' : fields SS.type} 
-            (HS' : relfs SS.subtype ss' ts') : fields expr :=
-            match HS' with
-            | Forall2_nil _ => []
-            | Forall2_cons s _ (conj _ Hst) Hssts =>
-                (fst s, EApp (translate_subtype Hst) (EPrj r (fst s))) :: (rechelp Hssts)
-            end in
-        EFun "r" (TRec (map (map_snd translate_type) ss)) (ERec (rechelp HS))
-    end.
-
-(* Coq is making me define this as a relation instead of a function... *)
-Inductive translate_subtype : forall {s t : SS.type}, 
-SS.subtype s t -> expr -> Prop :=
-    | ts_refl : forall (t : SS.type),
-        translate_subtype (SS.st_refl t)
-            (EFun "x" (translate_type t) (EVar "x"))
-    | ts_trans : forall (s u t : SS.type) (e1 e2 : expr)
-        (C1 : SS.subtype s u) (C2 : SS.subtype u t),
-        translate_subtype C1 e1 ->
-        translate_subtype C2 e2 ->
-        translate_subtype
-            (SS.st_trans s u t C1 C2)
-            (EFun "x" (translate_type s) 
-                (EApp e2 (EApp e1 (EVar "x"))))
-    | ts_top : forall (t : SS.type),
-        translate_subtype (SS.st_top t)
-            (EFun "x" (translate_type t) EUnit)
-    | ts_fun : forall (s1 t1 s2 t2 : SS.type) (e1 e2: expr)
-        (C1 : SS.subtype t1 s1) (C2 : SS.subtype s2 t2),
-        translate_subtype C1 e1 ->
-        translate_subtype C2 e2 ->
-        translate_subtype 
-            (SS.st_fun s1 t1 s2 t2 C1 C2)
-            (EFun "f" (translate_type (SS.TFun s1 s2 ))
-                ((EFun "x") (translate_type t1)
-                    (EApp e2 (EApp (EVar "f") (EApp e1 (EVar "x"))))))
-    | ts_rec_width : forall (us vs : fields SS.type),
-        translate_subtype
-            (SS.st_rec_width us vs)
-            (EFun "r" 
+    (* why Coq, why? I cannot define the translation
+        as a function from subtyping derivations 
+        to types... :( *)
+    Fail Fixpoint translate_subtype {u v : SST.type} (HS : SS.subtype u v) : expr :=
+        let x := EVar "x" in
+        let f := EVar "f" in
+        let r := EVar "r" in
+        match HS with
+        | SS.st_refl t => EFun "x" (translate_type t) x
+        | SS.st_trans s _ _ HSsu HSut => 
+            EFun "x" (translate_type s) 
+                (EApp (translate_subtype HSsu)
+                    (EApp (translate_subtype HSut) x))
+        | SS.st_top t => EFun "x" (translate_type t) EUnit
+        | SS.st_fun s1 s2 t1 _ C1 C2 =>
+            EFun "f" (translate_type (SST.TFun s1 s2 ))
+                (EFun "x" (translate_type t1) 
+                    (EApp (translate_subtype C2) 
+                        (EApp f
+                            (EApp (translate_subtype C1) x))))
+        | SS.st_rec_width us vs =>
+            EFun "r" 
                 (TRec (map (map_snd translate_type) (us ++ vs)))
                 (ERec 
                     (map 
                         (fun (u : field SS.type) => 
-                            (fst u, (EPrj (EVar "r") (fst u)))) 
-                        us)))
-    | ts_rec_depth : forall (ss ts : fields SS.type)
-        (HS : relfs SS.subtype ss ts) (es : fields expr),
-        map fst ss = map fst es ->
-        (forall (s : field SS.type) (t : field SS.type),
-        exists (H : SS.subtype (snd s) (snd t)),
-        In (s,t) (combine ss ts) ->
-        exists (e : field expr), translate_subtype H (snd e) /\
-        In (s,e) (combine ss es)) ->
-        translate_subtype
-            (SS.st_rec_depth ss ts HS)
-            (EFun "r" 
-                (TRec (map (map_snd translate_type) ss)) 
-                (ERec (map (fun e => 
-                    (fst e, EApp (snd e) (EPrj (EVar "r") (fst e)))) es)))
-    | ts_rec_perm : forall (ss ts : fields SS.type) (HP : perm ss ts),
-        translate_subtype 
-            (SS.st_rec_perm ss ts HP)
-            (EFun "r" 
-                (TRec (map (map_snd translate_type) ss))
-                (ERec 
-                    (map 
-                        (fun (lbl : field SS.type) => 
-                            (fst lbl, (EPrj (EVar "r") (fst lbl)))) 
-                        ss))).
+                            (fst u, (EPrj r (fst u)))) 
+                        us))
+        | SS.st_rec_depth ss _ HS =>
+            let fix rechelp {ss' ts' : fields SS.type} 
+                (HS' : relfs SS.subtype ss' ts') : fields expr :=
+                match HS' with
+                | Forall2_nil _ => []
+                | Forall2_cons s _ (conj _ Hst) Hssts =>
+                    (fst s, EApp (translate_subtype Hst) (EPrj r (fst s))) :: (rechelp Hssts)
+                end in
+            EFun "r" (TRec (map (map_snd translate_type) ss)) (ERec (rechelp HS))
+        end.
 
-Lemma translate_subtype_correct :
-    forall {s t : SS.type} (C : SS.subtype s t) (e : expr),
-    translate_subtype C e ->
-    forall (g : gamma),
-    check g e (TFun (translate_type s) (translate_type t)).
-Proof.
-    intros s t C e TST. dependent induction TST; intros g.
-    - constructor. constructor. reflexivity.
-    - remember (translate_type s) as s' in *.
-        remember (translate_type u) as u' in *.
-        remember (translate_type t) as t' in *.
-        constructor.
-        apply check_app with (t := u').
-        + apply IHTST2.
-        + apply check_app with (t := s').
-            * apply IHTST1.
-            * constructor. reflexivity.
-    - constructor. constructor.
-    - simpl. remember (translate_type s1) as s1' in *.
-        remember (translate_type s2) as s2' in *.
-        remember (translate_type t1) as t1' in *.
-        remember (translate_type t2) as t2' in *. 
-        constructor. constructor.
-        apply check_app with (t := s2').
-        + apply IHTST2.
-        + apply check_app with (t := s1');
-            try (constructor; reflexivity).
-            apply check_app with (t := t1');
-            try (constructor; reflexivity).
-            apply IHTST1.
-    - constructor. simpl. constructor.
-        induction us; constructor.
-        + destruct a as [a1 a2]; split; simpl;
-            try reflexivity.
-            apply check_prj with 
-                (ts := ((ID a1, translate_type a2)
-                    :: map (map_snd translate_type) (us ++ vs))).
-            * constructor. reflexivity.
-            * constructor. reflexivity.
-        + simpl. admit.
-            (* Requires a helper lemma for how adding 
-                field to a record type bound to a variable
-                in the context doesn't change
-                typing projections. *)
-    - constructor. constructor. admit.
-        (* requires a stronger induction 
-            hypothesis for translate_subtype. *)
-    - constructor. constructor.
-        fold translate_type.
-        dependent induction HP.
-        + constructor.
-        + destruct x as [x1 x2].
+    (* Coq is making me define this as a relation instead of a function... *)
+    Inductive translate_subtype : forall {s t : SST.type}, 
+    SS.subtype s t -> expr -> Prop :=
+        | ts_refl : forall (t : SST.type),
+            translate_subtype (SS.st_refl t)
+                (EFun "x" (translate_type t) (EVar "x"))
+        | ts_trans : forall (s u t : SST.type) (e1 e2 : expr)
+            (C1 : SS.subtype s u) (C2 : SS.subtype u t),
+            translate_subtype C1 e1 ->
+            translate_subtype C2 e2 ->
+            translate_subtype
+                (SS.st_trans s u t C1 C2)
+                (EFun "x" (translate_type s) 
+                    (EApp e2 (EApp e1 (EVar "x"))))
+        | ts_top : forall (t : SST.type),
+            translate_subtype (SS.st_top t)
+                (EFun "x" (translate_type t) EUnit)
+        | ts_fun : forall (s1 t1 s2 t2 : SST.type) (e1 e2: expr)
+            (C1 : SS.subtype t1 s1) (C2 : SS.subtype s2 t2),
+            translate_subtype C1 e1 ->
+            translate_subtype C2 e2 ->
+            translate_subtype 
+                (SS.st_fun s1 t1 s2 t2 C1 C2)
+                (EFun "f" (translate_type (SST.TFun s1 s2 ))
+                    ((EFun "x") (translate_type t1)
+                        (EApp e2 (EApp (EVar "f") (EApp e1 (EVar "x"))))))
+        | ts_rec_width : forall (us vs : fields SST.type),
+            translate_subtype
+                (SS.st_rec_width us vs)
+                (EFun "r" 
+                    (TRec (map (map_snd translate_type) (us ++ vs)))
+                    (ERec 
+                        (map 
+                            (fun (u : field SST.type) => 
+                                (fst u, (EPrj (EVar "r") (fst u)))) 
+                            us)))
+        | ts_rec_depth : forall (ss ts : fields SST.type)
+            (HS : relfs SS.subtype ss ts) (es : fields expr),
+            map fst ss = map fst es ->
+            (forall (s : field SST.type) (t : field SST.type),
+            exists (H : SS.subtype (snd s) (snd t)),
+            In (s,t) (combine ss ts) ->
+            exists (e : field expr), translate_subtype H (snd e) /\
+            In (s,e) (combine ss es)) ->
+            translate_subtype
+                (SS.st_rec_depth ss ts HS)
+                (EFun "r" 
+                    (TRec (map (map_snd translate_type) ss)) 
+                    (ERec (map (fun e => 
+                        (fst e, EApp (snd e) (EPrj (EVar "r") (fst e)))) es)))
+        | ts_rec_perm : forall (ss ts : fields SST.type) (HP : perm ss ts),
+            translate_subtype 
+                (SS.st_rec_perm ss ts HP)
+                (EFun "r" 
+                    (TRec (map (map_snd translate_type) ss))
+                    (ERec 
+                        (map 
+                            (fun (lbl : field SST.type) => 
+                                (fst lbl, (EPrj (EVar "r") (fst lbl)))) 
+                            ss))).
+
+    Lemma translate_subtype_correct :
+        forall {s t : SST.type} (C : SS.subtype s t) (e : expr),
+        translate_subtype C e ->
+        forall (g : gamma),
+        check g e (TFun (translate_type s) (translate_type t)).
+    Proof.
+        intros s t C e TST. dependent induction TST; intros g.
+        - constructor. constructor. reflexivity.
+        - remember (translate_type s) as s' in *.
+            remember (translate_type u) as u' in *.
+            remember (translate_type t) as t' in *.
             constructor.
-            * split; try reflexivity. simpl.
+            apply check_app with (t := u').
+            + apply IHTST2.
+            + apply check_app with (t := s').
+                * apply IHTST1.
+                * constructor. reflexivity.
+        - constructor. constructor.
+        - simpl. remember (translate_type s1) as s1' in *.
+            remember (translate_type s2) as s2' in *.
+            remember (translate_type t1) as t1' in *.
+            remember (translate_type t2) as t2' in *. 
+            constructor. constructor.
+            apply check_app with (t := s2').
+            + apply IHTST2.
+            + apply check_app with (t := s1');
+                try (constructor; reflexivity).
+                apply check_app with (t := t1');
+                try (constructor; reflexivity).
+                apply IHTST1.
+        - constructor. simpl. constructor.
+            induction us; constructor.
+            + destruct a as [a1 a2]; split; simpl;
+                try reflexivity.
                 apply check_prj with 
-                    (ts := ((ID x1, translate_type x2) 
-                        :: map (map_snd translate_type) l));
-                constructor; reflexivity.
-            * simpl. admit.
-            (* Requires a helper lemma for how adding 
-                field to a record type bound to a variable
-                in the context doesn't change
-                typing projections. *)
-        + destruct x as [x1 x2].
-            destruct y as [y1 y2].
-            constructor; simpl.
-            { split.
-                - admit.
-                    (* This case baffles me... *)
-                - simpl. apply check_prj with
-                    (ts := ((ID y1, translate_type y2)
-                    :: (ID x1, translate_type x2) 
-                        :: map (map_snd translate_type) l)).
-                    + constructor. admit.
-                        (* I don't understand 
-                            what is going on... *) 
-                    + constructor. reflexivity. }
-            { constructor.
-                - split; simpl.
-                    + admit.
-                        (* Why Coq, why? *)
-                    + apply check_prj with
-                        (ts := (ID y1, translate_type y2)
-                            :: (ID x1, translate_type x2) 
-                            :: map (map_snd translate_type) l).
-                        * admit.
-                            (* I don't get it... *)
-                        * constructor. reflexivity. }
-        + admit.
-            (* I don't feel like doing this... *)
-Admitted.
+                    (ts := ((ID a1, translate_type a2)
+                        :: map (map_snd translate_type) (us ++ vs))).
+                * constructor. reflexivity.
+                * constructor. reflexivity.
+            + simpl. admit.
+                (* Requires a helper lemma for how adding 
+                    field to a record type bound to a variable
+                    in the context doesn't change
+                    typing projections. *)
+        - constructor. constructor. admit.
+            (* requires a stronger induction 
+                hypothesis for translate_subtype. *)
+        - constructor. constructor.
+            fold translate_type.
+            dependent induction HP.
+            + constructor.
+            + destruct x as [x1 x2].
+                constructor.
+                * split; try reflexivity. simpl.
+                    apply check_prj with 
+                        (ts := ((ID x1, translate_type x2) 
+                            :: map (map_snd translate_type) l));
+                    constructor; reflexivity.
+                * simpl. admit.
+                (* Requires a helper lemma for how adding 
+                    field to a record type bound to a variable
+                    in the context doesn't change
+                    typing projections. *)
+            + destruct x as [x1 x2].
+                destruct y as [y1 y2].
+                constructor; simpl.
+                { split.
+                    - admit.
+                        (* This case baffles me... *)
+                    - simpl. apply check_prj with
+                        (ts := ((ID y1, translate_type y2)
+                        :: (ID x1, translate_type x2) 
+                            :: map (map_snd translate_type) l)).
+                        + constructor. admit.
+                            (* I don't understand 
+                                what is going on... *) 
+                        + constructor. reflexivity. }
+                { constructor.
+                    - split; simpl.
+                        + admit.
+                            (* Why Coq, why? *)
+                        + apply check_prj with
+                            (ts := (ID y1, translate_type y2)
+                                :: (ID x1, translate_type x2) 
+                                :: map (map_snd translate_type) l).
+                            * admit.
+                                (* I don't get it... *)
+                            * constructor. reflexivity. }
+            + admit.
+                (* I don't feel like doing this... *)
+    Admitted.
 
-Definition translate_gamma (g : @gamma SS.type) (x : id) :=
-    match g x with
-    | None => None
-    | Some t => Some (translate_type t)
-    end.
+    Definition translate_gamma (g : @gamma SST.type) (x : id) :=
+        match g x with
+        | None => None
+        | Some t => Some (translate_type t)
+        end.
 
-Lemma translate_gamma_bind :
-    forall (g : gamma) (x : id) (t : SS.type),
-    translate_gamma (bind x t g) = 
-        bind x (translate_type t) (translate_gamma g).
-Proof.
-    intros g x t. apply functional_extensionality.
-    intros y. unfold translate_gamma.
-    destruct (IdDec.eq_dec x y).
-    - subst. rewrite bind_correct.
-        rewrite bind_correct. reflexivity.
-    - unfold bind.
-        apply eqb_neq in n. rewrite n. reflexivity.
-Qed.
+    Lemma translate_gamma_bind :
+        forall (g : gamma) (x : id) (t : SST.type),
+        translate_gamma (bind x t g) = 
+            bind x (translate_type t) (translate_gamma g).
+    Proof.
+        intros g x t. apply functional_extensionality.
+        intros y. unfold translate_gamma.
+        destruct (IdDec.eq_dec x y).
+        - subst. rewrite bind_correct.
+            rewrite bind_correct. reflexivity.
+        - unfold bind.
+            apply eqb_neq in n. rewrite n. reflexivity.
+    Qed.
 
-Inductive translate_expr {g : @gamma SS.type} :
-forall {e : SS.expr} {t : SS.type},
-SS.check g e t -> expr -> Prop :=
-    | te_unit : 
-        forall (H : SS.check g SS.EUnit SS.TUnit),
-        translate_expr H EUnit
-    | te_var : forall (x : id) (t : SS.type) 
-        (H : SS.check g (SS.EVar x) t),
-        g x = Some t ->
-        translate_expr H (EVar x)
-    | te_fun : forall (x : id) (t1 t2 : SS.type) 
-        (e : SS.expr) (e' : expr)
-        (D2 : SS.check (bind x t1 g) e t2)
-        (H : SS.check g (SS.EFun x t1 e) (SS.TFun t1 t2)),
-        @translate_expr (bind x t1 g) e t2 D2 e' ->
-        translate_expr H (EFun x (translate_type t1) e')
-    | te_app : forall (e1 e2 : SS.expr) 
-        (t11 t12 : SS.type) (e1' e2' : expr)
-        (D1 : SS.check g e1 (SS.TFun t11 t12))
-        (D2 : SS.check g e2 t11)
-        (H : SS.check g (SS.EApp e1 e2) t12),
+    Inductive translate_expr {g : @gamma SST.type} :
+    forall {e : SSE.expr} {t : SST.type},
+    SS.check g e t -> expr -> Prop :=
+        | te_unit : 
+            forall (H : SS.check g SSE.EUnit SST.TUnit),
+            translate_expr H EUnit
+        | te_var : forall (x : id) (t : SST.type) 
+            (H : SS.check g (SSE.EVar x) t),
+            g x = Some t ->
+            translate_expr H (EVar x)
+        | te_fun : forall (x : id) (t1 t2 : SST.type) 
+            (e : SSE.expr) (e' : expr)
+            (D2 : SS.check (bind x t1 g) e t2)
+            (H : SS.check g (SSE.EFun x t1 e) (SST.TFun t1 t2)),
+            @translate_expr (bind x t1 g) e t2 D2 e' ->
+            translate_expr H (EFun x (translate_type t1) e')
+        | te_app : forall (e1 e2 : SSE.expr) 
+            (t11 t12 : SST.type) (e1' e2' : expr)
+            (D1 : SS.check g e1 (SST.TFun t11 t12))
+            (D2 : SS.check g e2 t11)
+            (H : SS.check g (SSE.EApp e1 e2) t12),
+            translate_expr D1 e1' ->
+            translate_expr D2 e2' ->
+            translate_expr H (EApp e1' e2')
+        (* Skipping translation for records...for now! *)
+        | te_prj : forall (e : SSE.expr) (x : id) 
+            (t : SST.type) (ts : fields SST.type) (e' : expr)
+            (D1 : SS.check g e (SST.TRec ts))
+            (H : SS.check g (SSE.EPrj e x) t),
+            In (x,t) ts ->
+            translate_expr D1 e' ->
+            translate_expr H (EPrj e' x)
+        | te_subsume : forall (e : SSE.expr) (s t : SST.type) (d' c' : expr)
+            (D : SS.check g e s) (C : SS.subtype s t)
+            (H : SS.check g e t),
+            translate_subtype C c' ->
+            translate_expr D d' ->
+            translate_expr H (EApp c' d').
+
+    Theorem translate_expr_correct :
+        forall {g : @gamma SST.type} {e : SSE.expr} {t : SST.type}
+        (D : SS.check g e t) (e' : expr),
+        translate_expr D e' -> 
+        check (translate_gamma g) e' (translate_type t).
+    Proof.
+        intros g e t D e' TE. 
+            dependent induction TE.
+        - constructor.
+        - constructor. unfold translate_gamma.
+            rewrite H0. reflexivity.
+        - constructor. fold translate_type.
+            rewrite <- translate_gamma_bind.
+            assumption.
+        - simpl in *. remember (translate_type t11) as t11' in *.
+            remember (translate_type t12) as t12' in *.
+            apply check_app with (t := t11'); assumption.
+        - simpl in *.
+            remember (map (map_snd translate_type) ts) as ts' in *.
+            apply check_prj with (ts := ts'); auto. subst.
+            assert (dumb : (x, translate_type t)
+                = (map_snd translate_type) (x,t));
+            try reflexivity.
+            rewrite dumb. apply in_map. assumption.
+        - remember (translate_type s) as s' in *.
+            remember (translate_type t) as t' in *.
+            apply check_app with (t := s'); auto. subst. 
+            apply translate_subtype_correct with (C0 := C).
+            assumption.
+    Qed.
+
+    (* Below definition is incorrect :
+        e1' and e2' should evaluate to
+        the same value but they may not be equal *)
+    Theorem Coherence :
+        forall {g : @gamma SST.type} {e : SSE.expr} {t : SST.type}
+        (D1 D2 : SS.check g e t) (e1' e2' : expr),
         translate_expr D1 e1' ->
-        translate_expr D2 e2' ->
-        translate_expr H (EApp e1' e2')
-    (* Skipping translation for records...for now! *)
-    | te_prj : forall (e : SS.expr) (x : id) 
-        (t : SS.type) (ts : fields SS.type) (e' : expr)
-        (D1 : SS.check g e (SS.TRec ts))
-        (H : SS.check g (SS.EPrj e x) t),
-        In (x,t) ts ->
-        translate_expr D1 e' ->
-        translate_expr H (EPrj e' x)
-    | te_subsume : forall (e : SS.expr) (s t : SS.type) (d' c' : expr)
-        (D : SS.check g e s) (C : SS.subtype s t)
-        (H : SS.check g e t),
-        translate_subtype C c' ->
-        translate_expr D d' ->
-        translate_expr H (EApp c' d').
+        translate_expr D2 e2' -> e1' = e2'.
+    Proof.
+    Abort.
+End Coercion.
 
-Theorem translate_expr_correct :
-    forall {g : @gamma SS.type} {e : SS.expr} {t : SS.type}
-    (D : SS.check g e t) (e' : expr),
-    translate_expr D e' -> 
-    check (translate_gamma g) e' (translate_type t).
+Module AlgorithmicSubtyping.
+Module SS := SubsumptionSTLC.
+Import SS.SSType.
+Import SS.SSExpr.
+Import SS.Step.
+
+Inductive subtype : type -> type -> Prop :=
+    | st_top : forall (s : type), subtype s TTop
+    | st_unit : subtype TUnit TUnit
+    | st_fun : forall (s1 s2 t1 t2 : type),
+        subtype t1 s1 ->
+        subtype s2 t2 ->
+        subtype (TFun s1 s2) (TFun t1 t2)
+    | st_rec : forall (ss ts : fields type),
+        (forall (t : field type),
+        In t ts -> 
+        exists (s : field type),
+        In s ss /\ relf subtype s t) ->
+        subtype (TRec ss) (TRec ts).
+
+Lemma Reflexive :
+    forall (t : type),
+    subtype t t.
 Proof.
-    intros g e t D e' TE. 
-        dependent induction TE.
-    - constructor.
-    - constructor. unfold translate_gamma.
-        rewrite H0. reflexivity.
-    - constructor. fold translate_type.
-        rewrite <- translate_gamma_bind.
-        assumption.
-    - simpl in *. remember (translate_type t11) as t11' in *.
-        remember (translate_type t12) as t12' in *.
-        apply check_app with (t := t11'); assumption.
-    - simpl in *.
-        remember (map (map_snd translate_type) ts) as ts' in *.
-        apply check_prj with (ts := ts'); auto. subst.
-        assert (dumb : (x, translate_type t)
-            = (map_snd translate_type) (x,t));
-        try reflexivity.
-        rewrite dumb. apply in_map. assumption.
-    - remember (translate_type s) as s' in *.
-        remember (translate_type t) as t' in *.
-        apply check_app with (t := s'); auto. subst. 
-        apply translate_subtype_correct with (C0 := C).
-        assumption.
+    intros t. induction t using IHType;
+    constructor; auto.
+    intros t Hin. exists t. split; auto.
+    pose proof Forall_forall 
+        (predf (fun t => subtype t t)) fs as FF.
+    unfold predfs in H. destruct FF as [F1 _].
+    apply F1 with (x := t) in H; auto.
+    split; auto.
 Qed.
 
-(* Below definition is incorrect :
-    e1' and e2' should evaluate to
-    the same value but they may not be equal *)
-Theorem Coherence :
-    forall {g : @gamma SS.type} {e : SS.expr} {t : SS.type}
-    (D1 D2 : SS.check g e t) (e1' e2' : expr),
-    translate_expr D1 e1' ->
-    translate_expr D2 e2' -> e1' = e2'.
+Lemma Transitive :
+    forall (s u t : type),
+    subtype s u -> subtype u t -> subtype s t.
 Proof.
-    intros g e t D1 D2 e1' e2' TE1.
-    induction TE1; intros TE2.
-    - apply translate_expr_correct in TE2 as TEC2.
-        simpl in *. inv TEC2; auto.
-        + admit.
-Admitted.
-End Coercion.
+    intros s u t Hsu.
+    generalize dependent t.
+    dependent induction Hsu;
+    intros t Hut.
+    - inv Hut; constructor.
+    - inv Hut; constructor.
+    - inv Hut; constructor;
+        apply IHHsu2 in H3; auto.
+        admit.
+        (* Induction hypothesis for 
+            s1 is backwards. *)
+    - inv Hut; constructor.
+        intros t Hints0.
+        apply H1 in Hints0 as 
+        [s [Hints HSst]].
+        apply H in Hints as
+        [u [Hinss HRst]].
+        exists u. split; auto.
+        admit.
+        (* Induction hypothesis
+            is not strong enough. *)
+Admitted. 
+
+Theorem Complete :
+    forall (s t : type),
+    SS.subtype s t -> subtype s t.
+Proof.
+    intros s t HS.
+    dependent induction HS using SS.IHSubtype.
+    - apply Reflexive.
+    - apply Transitive with (u := u); auto.
+    - constructor.
+    - constructor; auto.
+    - constructor. intros t Hintus.
+        exists t. split.
+        + apply in_or_app. left.
+            assumption.
+        + split; auto.
+            apply Reflexive.
+    - constructor. intros t Hinvs.
+        apply relfs_in_exists_r with (vs0 := vs); auto.
+    - constructor. intros t Hinvs.
+        exists t. split.
+        + apply Permutation_in with (l := vs); auto.
+            apply Permutation_sym; auto.
+        + split; auto. apply Reflexive.
+Qed.
+End AlgorithmicSubtyping.
